hungarian best even neighbour

Hungarian_Method/Primal_Dual_Path_Search.thy
@@ -1,25 +1,2048 @@
 theory Primal_Dual_Path_Search
   imports Berge_Lemma.Berge Flow_Theory.Arith_Lemmas "HOL-Data_Structures.Set_Specs"
 "HOL-Data_Structures.Map_Specs"
+RANKING.More_Graph
 begin
+(*TODO MOVE*)
+lemma pair_eq_fst_snd_eq:
+      "(a, b) = c \<Longrightarrow> a = fst c"
+      "(a, b) = c \<Longrightarrow> b = snd c"
+  by auto
 
-record ('forest, 'seen, 'slack, 'potential,'gimpl) primal_dual_state = 
-new_to_left_seen::'seen
+lemma walk_reflexive_cong: "\<lbrakk>u \<in> Vs G; u = u'; u' = u''\<rbrakk> \<Longrightarrow> walk_betw G u [u'] u''"
+  using walk_reflexive by simp
+
+lemma bipartite_even_and_odd_walk:
+  assumes "bipartite G X Y" "x \<in> X"
+          "walk_betw G x p y"
+    shows "odd (length p) \<Longrightarrow> y \<in> X"
+          "even (length p) \<Longrightarrow> y \<in> Y"
+proof-
+  have "(odd (length p) \<longrightarrow> y \<in> X) \<and> (even (length p) \<longrightarrow> y \<in> Y)"
+    using assms(3)
+  proof(induction p arbitrary: y rule: rev_induct)
+    case Nil
+    then show ?case by(simp add: walk_betw_def)
+  next
+    case (snoc x' xs)
+    note IH = this
+    show ?case 
+    proof(cases "even (length (xs@[x]))")
+      case True
+      hence odd: "odd (length xs)" by simp
+      have "\<exists> y'. walk_betw G x xs y' \<and> {y', y} \<in> G"
+        using odd snoc(2) path_2[of G y] path_suff[of G _ "[_, y]"] snoc.prems[simplified walk_betw_def] 
+        by(cases xs rule: rev_cases)
+          (auto intro!: exI[of _ "last xs"] walk_reflexive_cong simp add: walk_pref)
+      then obtain y' where y':"walk_betw G x xs y'" "{y', y} \<in> G"
+        by auto
+      moreover hence "y' \<in> X" 
+        using snoc(1) odd by simp
+      ultimately have "y \<in> Y"
+        using assms(1) bipartite_edgeD(1) by fastforce
+      thus ?thesis
+        using True by fastforce
+    next
+      case False
+      show ?thesis
+      proof(cases xs rule: rev_cases)
+        case Nil
+        hence "y = x" 
+          using IH(2) snoc.prems[simplified walk_betw_def]  
+          by auto
+        then show ?thesis 
+          by (simp add: assms(2) local.Nil)
+      next
+        case (snoc list a)
+      hence even: "even (length xs)"using False  by simp
+      have "\<exists> y'. (walk_betw G x xs y' \<and> {y', y} \<in> G)"
+        using IH(2)  path_suff[of G _ "[_, y]"] 
+             snoc.prems[simplified walk_betw_def] 
+        by(auto intro!: exI[of _ a] simp add: snoc walk_pref)
+      then obtain y' where y':"walk_betw G x xs y'" "{y', y} \<in> G"
+        by auto
+      moreover hence "y' \<in> Y" 
+        using IH(1) even by simp
+      ultimately have "y \<in> X"
+        using assms(1) bipartite_edgeD(2) by fastforce
+      thus ?thesis
+        using False by fastforce
+    qed
+  qed
+qed
+  thus  "odd (length p) \<Longrightarrow> y \<in> X" "even (length p) \<Longrightarrow> y \<in> Y" 
+    by auto
+qed
+
+lemma finite_G_finite_f_of_edge_verts:
+"finite G \<Longrightarrow> finite {f x y | x y. {x, y} \<in> G}"
+proof(induction G rule: finite_induct)
+  case (insert e F)
+  show ?case 
+  proof(cases "\<exists> x y. e = {x, y}")
+    case True
+    then obtain x y where "e = {x, y}" by auto
+    hence "{f x y | x y. {x, y} \<in> insert e F} = 
+           {f x y | x y. {x, y} \<in> F} \<union> {f x y, f y x}" 
+      by (auto simp add: doubleton_eq_iff)
+    then show ?thesis 
+      using insert by simp
+  next
+    case False
+  hence "{f x y | x y. {x, y} \<in> insert e F} = 
+           {f x y | x y. {x, y} \<in> F}" by auto
+  then show ?thesis
+    using insert by simp
+  qed
+qed simp
+ 
+
+lemma add_non_min_element_Min:
+"finite A \<Longrightarrow> A \<noteq> {} \<Longrightarrow> y \<le> x \<Longrightarrow> y \<in> A\<Longrightarrow> B = insert x A \<Longrightarrow> Min B = Min A"
+  by (metis Min.boundedE Min.insert_not_elem insert_absorb min_def order_antisym)
+(*TOTO MOVE*)
+lemma conj_intro:"\<lbrakk>P1;P2;P3;P4;P5;P6\<rbrakk> \<Longrightarrow> P1 \<and> P2 \<and> P3 \<and> P4 \<and> P5 \<and>P6" for P1 P2 P3 P4 P5 P6
+      by simp
+lemma conjD:"P1 \<and> P2 \<and> P3 \<and> P4 \<and> P5 \<and>P6 \<Longrightarrow> P1"
+               "P1 \<and> P2 \<and> P3 \<and> P4 \<and> P5 \<and>P6 \<Longrightarrow> P2"
+               "P1 \<and> P2 \<and> P3 \<and> P4 \<and> P5 \<and>P6 \<Longrightarrow> P3"
+               "P1 \<and> P2 \<and> P3 \<and> P4 \<and> P5 \<and>P6 \<Longrightarrow> P4"
+               "P1 \<and> P2 \<and> P3 \<and> P4 \<and> P5 \<and>P6  \<Longrightarrow> P5"
+                "P1 \<and> P2 \<and> P3 \<and> P4 \<and> P5 \<and>P6  \<Longrightarrow> P6"for P1 P2 P3 P4 P5 P6
+      by auto
+(*
+definition semibipartite :: "'a graph \<Rightarrow> 'a set \<Rightarrow> 'a set \<Rightarrow> bool" where
+  "semibipartite G X Y  = ( X \<inter> Y = {} \<and> (\<forall>e \<in> G. \<not> e \<subseteq> X))"
+*)
+record ('forest, 'ben, 'heap, 'miss, 'v) hungarian_search_state = 
 forest::'forest
-seen::'seen
-slack::'slack
-potential::'potential
-tight_graph::'gimpl
-
+best_even_neighbour::'ben
+heap::'heap
+missed::'miss
+acc::real
+augpath::"('v list) option"
+(*
 datatype ('v, 'seen, 'forest) path_or_forest = Path "'v list"
   | Forest 'seen 'forest
-
+*)
 locale primal_dual_path_search_spec = 
   fixes G::"'v set set"
+    and edge_costs::"'v \<Rightarrow> 'v \<Rightarrow> real"
+    and left::'vset
+    and right::'vset
+    and in_G::"'v \<Rightarrow> 'v \<Rightarrow> bool"
+    and right_neighbs::"'v \<Rightarrow> 'vset"
+
     and buddy::"'v \<Rightarrow> 'v option"
-    and get_path_or_extend_forest:: 
-       "'gimpl \<Rightarrow> 'vset \<Rightarrow> 'vset \<Rightarrow>'forest \<Rightarrow> ('v \<Rightarrow> 'v option)
-          \<Rightarrow> ('v, 'vset, 'forest) path_or_forest"
+
+    and extend_forest_even_unclassified::
+        "'forest \<Rightarrow> 'v \<Rightarrow> 'v \<Rightarrow> 'v \<Rightarrow> 'forest"
+    and evens::"'forest \<Rightarrow> 'vset"
+    and odds::"'forest \<Rightarrow> 'vset"
+    and get_path::"'forest \<Rightarrow> 'v \<Rightarrow> 'v list"
+    and abstract_forest::"'forest \<Rightarrow> 'v set set"
+    and empty_forest::"'vset \<Rightarrow> 'forest"
+    and forest_invar::"'v set set \<Rightarrow> 'forest \<Rightarrow> bool"
+    and roots::"'forest \<Rightarrow> 'vset"
+
+   and potential_upd::"'potential \<Rightarrow> 'v \<Rightarrow> real \<Rightarrow> 'potential"
+   and potential_lookup::"'potential \<Rightarrow> 'v \<Rightarrow> real option"
+   and potential_invar::"'potential \<Rightarrow> bool"
+   and initial_pot::"'potential"
+
+   and ben_empty::'ben
+   and ben_lookup::"'ben \<Rightarrow> 'v \<Rightarrow> 'v option"
+   and ben_upd::"'ben \<Rightarrow> 'v \<Rightarrow> 'v \<Rightarrow> 'ben"
+   and ben_invar::"'ben \<Rightarrow> bool"
+
+   and heap_empty::'heap
+   and heap_extract_min::"'heap \<Rightarrow> ('heap \<times> 'v option)"
+   and heap_decrease_key::"'heap \<Rightarrow> 'v \<Rightarrow> real \<Rightarrow> 'heap"
+   and heap_insert::"'heap \<Rightarrow> 'v \<Rightarrow> real \<Rightarrow> 'heap"
+   and heap_invar::"'heap \<Rightarrow> bool"
+   and heap_abstract::"'heap \<Rightarrow> ('v \<times> real) set"
+
+   and missed_empty::'miss
+   and missed_lookup::"'miss \<Rightarrow> 'v \<Rightarrow> real option"
+   and missed_upd::"'miss \<Rightarrow> 'v \<Rightarrow> real \<Rightarrow> 'miss"
+   and missed_invar::"'miss \<Rightarrow> bool"
+
+   and to_list::"'vset \<Rightarrow> 'v list"
+   and vset_to_set::"'vset \<Rightarrow> 'v set"
+   and vset_isin::"'v \<Rightarrow> 'vset \<Rightarrow> bool"
+   and vset_empty::"'vset"
+   and vset_insert::"'v \<Rightarrow> 'vset \<Rightarrow> 'vset"
+   and vset_invar::"'vset \<Rightarrow> bool"
+begin
+
+notation edge_costs ("\<w>")
+
+abbreviation "aevens state \<equiv> vset_to_set (evens (forest state))"
+abbreviation "aodds state \<equiv> vset_to_set (odds (forest state))"
+abbreviation "missed_at state v \<equiv> abstract_real_map (missed_lookup (missed state)) v"
+abbreviation "\<pi> v \<equiv> abstract_real_map (potential_lookup initial_pot) v"
+abbreviation "\<F> state \<equiv> abstract_forest (forest state)"
+abbreviation "L  \<equiv> vset_to_set left"
+abbreviation "R  \<equiv> vset_to_set right"
+
+definition "\<M> = {{u, v} | u v. Some v = buddy u}"
+
+definition "w\<^sub>\<pi> u v = edge_costs u v - \<pi> u - \<pi> v"
+
+definition "invar_basic state= 
+  (forest_invar \<M> (forest state) \<and>
+    ben_invar (best_even_neighbour state) \<and>
+    heap_invar (heap state) \<and>
+    missed_invar (missed state) \<and>
+    \<F> state \<subseteq> G \<and>
+    dom (ben_lookup (best_even_neighbour state)) \<subseteq> Vs G \<and>
+    dom (missed_lookup (missed state)) \<subseteq> Vs G \<and>
+     fst ` heap_abstract (heap state) \<subseteq> Vs G \<and>
+     aevens state \<subseteq> L \<and> aodds state \<subseteq> R)"
+
+lemma invar_basicE:
+"invar_basic state \<Longrightarrow>
+(\<lbrakk>forest_invar \<M> (forest state);
+  ben_invar (best_even_neighbour state);
+  heap_invar (heap state);
+  missed_invar (missed state);\<F> state \<subseteq> G;
+  dom (ben_lookup (best_even_neighbour state)) \<subseteq> Vs G;
+  dom (missed_lookup (missed state)) \<subseteq> Vs G;
+  fst ` heap_abstract (heap state) \<subseteq> Vs G;
+  aevens state \<subseteq> L; aodds state \<subseteq> R\<rbrakk> 
+ \<Longrightarrow> P)
+\<Longrightarrow> P"
+and invar_basicI:
+"\<lbrakk>forest_invar \<M> (forest state);
+  ben_invar (best_even_neighbour state);
+  heap_invar (heap state);
+  missed_invar (missed state);\<F> state \<subseteq> G;
+  dom (ben_lookup (best_even_neighbour state)) \<subseteq> Vs G;
+  dom (missed_lookup (missed state)) \<subseteq> Vs G;
+  fst ` heap_abstract (heap state) \<subseteq> Vs G;
+  aevens state \<subseteq> L; aodds state \<subseteq> R\<rbrakk> 
+ \<Longrightarrow> invar_basic state"
+and invar_basicD:
+"invar_basic state \<Longrightarrow> forest_invar \<M> (forest state)"
+"invar_basic state \<Longrightarrow> ben_invar (best_even_neighbour state)"
+"invar_basic state \<Longrightarrow> heap_invar (heap state)"
+"invar_basic state \<Longrightarrow> missed_invar (missed state)"
+"invar_basic state \<Longrightarrow> \<F> state \<subseteq> G"
+"invar_basic state \<Longrightarrow> dom (ben_lookup (best_even_neighbour state)) \<subseteq> Vs G"
+"invar_basic state \<Longrightarrow> dom (missed_lookup (missed state)) \<subseteq> Vs G"
+"invar_basic state \<Longrightarrow> fst ` heap_abstract (heap state) \<subseteq> Vs G"
+"invar_basic state \<Longrightarrow> aevens state \<subseteq> L"
+"invar_basic state \<Longrightarrow> aodds state \<subseteq> R"
+  by(auto simp add: invar_basic_def)
+
+definition working_potential ("\<pi>\<^sup>*") where
+"\<pi>\<^sup>* state v =
+        (if vset_isin v (evens (forest state)) then 
+           \<pi> v + acc state - missed_at state v
+         else if vset_isin v (odds (forest state)) then 
+           \<pi> v - acc state + missed_at state v
+         else \<pi> v)"
+
+definition "invar_feasible_potential state =
+            (\<forall> u v. {u, v} \<in> G \<longrightarrow>
+               edge_costs u v \<ge> \<pi>\<^sup>* state u + \<pi>\<^sup>* state v)"
+
+lemma invar_feasible_potentialE:
+"invar_feasible_potential state \<Longrightarrow>
+((\<And> u v. {u, v} \<in> G \<Longrightarrow>
+               edge_costs u v \<ge> \<pi>\<^sup>* state u + \<pi>\<^sup>* state v) \<Longrightarrow> P)
+\<Longrightarrow> P"
+and invar_feasible_potentialI:
+"(\<And> u v. {u, v} \<in> G \<Longrightarrow>
+               edge_costs u v \<ge> \<pi>\<^sup>* state u + \<pi>\<^sup>* state v) 
+\<Longrightarrow> invar_feasible_potential state"
+and invar_feasible_potentialD:
+"\<lbrakk>invar_feasible_potential state;  {u, v} \<in> G\<rbrakk>
+   \<Longrightarrow> edge_costs u v \<ge> \<pi>\<^sup>* state u + \<pi>\<^sup>* state v"
+  by (auto simp add: invar_feasible_potential_def)
+
+definition "invar_forest_tight state = 
+            (\<forall> e \<in> \<F> state.
+               \<exists> u v. edge_costs u v = \<pi>\<^sup>* state u + \<pi>\<^sup>* state v)"
+
+lemma invar_forest_tightE:
+"invar_forest_tight state \<Longrightarrow>
+ ((\<And> e. e \<in> \<F> state \<Longrightarrow>
+               \<exists> u v. edge_costs u v = \<pi>\<^sup>* state u + \<pi>\<^sup>* state v) \<Longrightarrow> P)
+\<Longrightarrow> P"
+and invar_forest_tightI:
+"(\<And> e. e \<in> \<F> state \<Longrightarrow>
+               \<exists> u v. edge_costs u v = \<pi>\<^sup>* state u + \<pi>\<^sup>* state v)
+ \<Longrightarrow> invar_forest_tight state"
+and invar_forest_tightD:
+"\<lbrakk>invar_forest_tight state;  e \<in> \<F> state\<rbrakk> 
+  \<Longrightarrow> \<exists> u v. edge_costs u v = \<pi>\<^sup>* state u + \<pi>\<^sup>* state v"
+  by(auto simp add: invar_forest_tight_def)
+
+definition "invar_matching_tight state = 
+            (\<forall> u v. {u, v} \<in> \<M> \<longrightarrow>
+               edge_costs u v = \<pi>\<^sup>* state u + \<pi>\<^sup>* state v)"
+
+lemma invar_matching_tightE:
+"invar_matching_tight state \<Longrightarrow>
+((\<And> u v. {u, v} \<in> \<M> \<Longrightarrow>
+               edge_costs u v = \<pi>\<^sup>* state u + \<pi>\<^sup>* state v) \<Longrightarrow> P)
+\<Longrightarrow> P"
+and invar_matching_tightI:
+"(\<And> u v. {u, v} \<in> \<M> \<Longrightarrow>
+               edge_costs u v = \<pi>\<^sup>* state u + \<pi>\<^sup>* state v)
+ \<Longrightarrow> invar_matching_tight state"
+and invar_matching_tightD:
+"\<lbrakk>invar_matching_tight state; {u, v} \<in> \<M>\<rbrakk> \<Longrightarrow>
+               edge_costs u v = \<pi>\<^sup>* state u + \<pi>\<^sup>* state v"
+  by(auto simp add: invar_matching_tight_def)
+
+definition "invar_best_even_neighbour_heap state =
+  (heap_abstract (heap state) = 
+   {(r, k) | r k. r \<in> Vs G - aevens state - aodds state \<and>
+                  (\<exists> l. k = w\<^sub>\<pi> l r + missed_at state l \<and>
+                       ben_lookup (best_even_neighbour state) r = Some l)})"
+
+lemma invar_best_even_neighbour_heapE:
+"invar_best_even_neighbour_heap state \<Longrightarrow>
+(heap_abstract (heap state) = 
+   {(r, k) | r k. r \<in> Vs G - aevens state - aodds state \<and>
+                  (\<exists> l. k = w\<^sub>\<pi> l r + missed_at state l \<and>
+                       ben_lookup (best_even_neighbour state) r = Some l)}
+ \<Longrightarrow> P)
+\<Longrightarrow>P"
+and invar_best_even_neighbour_heapI:
+"heap_abstract (heap state) = 
+   {(r, k) | r k. r \<in> Vs G - aevens state - aodds state \<and>
+                 (\<exists> l. k = w\<^sub>\<pi> l r + missed_at state l \<and>
+                       ben_lookup (best_even_neighbour state) r = Some l)}
+ \<Longrightarrow> invar_best_even_neighbour_heap state"
+and invar_best_even_neighbour_heapD:
+"invar_best_even_neighbour_heap state \<Longrightarrow>
+heap_abstract (heap state) = 
+   {(r, k) | r k. r \<in> Vs G - aevens state - aodds state \<and>
+                  (\<exists> l. k = w\<^sub>\<pi> l r + missed_at state l \<and>
+                       ben_lookup (best_even_neighbour state) r = Some l)}"
+  by(auto simp add: invar_best_even_neighbour_heap_def)
+
+definition "invar_best_even_neighbour_map state = 
+     (\<forall> r \<in> Vs G - aevens state - aodds state.
+           ((\<nexists> l. l \<in> aevens state \<and> {l, r} \<in> G) 
+                  \<longrightarrow> ben_lookup (best_even_neighbour state) r = None)
+          \<and>((\<exists> l. l \<in> aevens state \<and> {l, r} \<in> G)
+                  \<longrightarrow> (\<exists> l. ben_lookup (best_even_neighbour state) r = Some l \<and>
+                            {r, l} \<in> G  \<and>  l \<in> aevens state \<and>
+                            w\<^sub>\<pi> l r + missed_at state l = 
+                            Min {w\<^sub>\<pi> l r + missed_at state l | l. 
+                                   l \<in> aevens state \<and> {l, r} \<in> G})))"
+
+lemma invar_best_even_neighbour_mapE:
+"invar_best_even_neighbour_map state \<Longrightarrow>
+(\<lbrakk>(\<And> r. \<lbrakk> r \<in> Vs G; r \<notin>  aevens state; r \<notin> aodds state;
+         \<nexists> l. l \<in> aevens state \<and> {l, r} \<in> G \<rbrakk> 
+      \<Longrightarrow> ben_lookup (best_even_neighbour state) r = None);
+  (\<And> r. \<lbrakk> r \<in> Vs G; r \<notin>  aevens state; r \<notin> aodds state;
+         \<exists> l. l \<in> aevens state \<and> {l, r} \<in> G \<rbrakk> 
+      \<Longrightarrow> (\<exists> l. ben_lookup (best_even_neighbour state) r = Some l \<and>
+                            {r, l} \<in> G  \<and>  l \<in> aevens state \<and>
+                            w\<^sub>\<pi> l r + missed_at state l = 
+                            Min {w\<^sub>\<pi> l r + missed_at state l | l. 
+                                   l \<in> aevens state \<and> {l, r} \<in> G}))\<rbrakk>
+  \<Longrightarrow> P)
+\<Longrightarrow> P"
+and invar_best_even_neighbour_mapI:
+"\<lbrakk>(\<And> r. \<lbrakk> r \<in> Vs G; r \<notin>  aevens state; r \<notin> aodds state;
+         \<nexists> l. l \<in> aevens state \<and> {l, r} \<in> G \<rbrakk> 
+      \<Longrightarrow> ben_lookup (best_even_neighbour state) r = None);
+  (\<And> r. \<lbrakk> r \<in> Vs G; r \<notin>  aevens state; r \<notin> aodds state;
+         \<exists> l. l \<in> aevens state \<and> {l, r} \<in> G \<rbrakk> 
+      \<Longrightarrow> (\<exists> l. ben_lookup (best_even_neighbour state) r = Some l \<and>
+                            {r, l} \<in> G  \<and>  l \<in> aevens state \<and>
+                            w\<^sub>\<pi> l r + missed_at state l = 
+                            Min {w\<^sub>\<pi> l r + missed_at state l | l. 
+                                   l \<in> aevens state \<and> {l, r} \<in> G}))\<rbrakk>
+  \<Longrightarrow> invar_best_even_neighbour_map state"
+and invar_best_even_neighbour_mapD:
+"\<lbrakk>invar_best_even_neighbour_map state ; r \<in> Vs G; 
+  r \<notin>  aevens state; r \<notin> aodds state; \<nexists> l. l \<in> aevens state \<and> {l, r} \<in> G \<rbrakk> 
+      \<Longrightarrow> ben_lookup (best_even_neighbour state) r = None"
+"\<lbrakk>invar_best_even_neighbour_map state; r \<in> Vs G; 
+  r \<notin>  aevens state; r \<notin> aodds state;\<exists> l. l \<in> aevens state \<and> {l, r} \<in> G \<rbrakk> 
+      \<Longrightarrow> (\<exists> l. ben_lookup (best_even_neighbour state) r = Some l \<and>
+                            {r, l} \<in> G  \<and>  l \<in> aevens state \<and>
+                            w\<^sub>\<pi> l r + missed_at state l = 
+                            Min {w\<^sub>\<pi> l r + missed_at state l | l. 
+                                   l \<in> aevens state \<and> {l, r} \<in> G})"
+  by(auto simp add: invar_best_even_neighbour_map_def)
+
+definition "edge_slack pot x y = 
+    edge_costs x y - pot x - pot y"
+
+(*definition "add_to_pot pot x val = 
+           (case potential_lookup pot x of 
+             None \<Rightarrow> potential_upd pot x val 
+             | Some val' \<Rightarrow> potential_upd pot x (val + val'))"*)
+(*
+definition "best_even_neighbour_ereal_costs ben off r = (
+            case (ben_lookup ben r) of None \<Rightarrow> PInfty|
+             Some l \<Rightarrow> w\<^sub>\<pi> l r - off)"*)
+(*
+definition "best_even_neighbour_costs ben v = snd (the (ben_lookup ben v))"
+*)(*
+lemma best_even_neighbour_real_and_ereal_costs:
+ "(ben_lookup ben v) \<noteq> None \<Longrightarrow>
+  best_even_neighbour_ereal_costs ben v = best_even_neighbour_costs ben v"
+  by(auto simp add: best_even_neighbour_ereal_costs_def
+                    best_even_neighbour_costs_def
+        split: option.split)
+*)
+definition "update_best_even_neighbour off ben queue l =
+   foldl 
+       (\<lambda> (ben, queue) r. 
+                (case ben_lookup ben r of None \<Rightarrow>
+                     (ben_upd ben r l, heap_insert queue r (w\<^sub>\<pi> l r + off l)) |
+                 Some l' \<Rightarrow>
+                 if w\<^sub>\<pi> l r + off l < w\<^sub>\<pi> l' r + off l'
+                 then (ben_upd ben r l, heap_decrease_key queue r (w\<^sub>\<pi> l r + off l))
+                 else (ben, queue)))
+                   (ben, queue) 
+        (to_list (right_neighbs l))"
+
+definition "update_best_even_neighbours off ben queue new_evens =
+  foldl 
+    (\<lambda> ben_queue r. update_best_even_neighbour off (fst ben_queue) (snd ben_queue) r) 
+  (ben, queue) new_evens"
+(*
+definition "find_next_edge ben queue= 
+             (foldl (\<lambda> result v. 
+                 if vset_isin v odd_verts then result
+                 else
+                  (case ben_lookup ben v of None \<Rightarrow> result
+                     | Some (e, sl) => 
+                     (case result of None \<Rightarrow> Some (e, v, sl)
+                         | Some (x, y, \<epsilon>) \<Rightarrow> 
+                             (if sl < \<epsilon> then Some (e, v, sl)
+                                 else Some (x, y, \<epsilon>))))
+                    ) None (to_list right))"
+*)
+definition "unmatched_lefts = filter (\<lambda> v. if buddy v = None then True else False) (to_list left)"
+definition "forest_roots = foldl (\<lambda> vset v. vset_insert v vset) vset_empty unmatched_lefts"
+definition "init_best_even_neighbour = 
+   update_best_even_neighbours (\<lambda> x. 0) ben_empty heap_empty unmatched_lefts"
+
+definition "initial_state = 
+ \<lparr>forest= empty_forest forest_roots, 
+  best_even_neighbour= fst (init_best_even_neighbour),
+  heap = snd (init_best_even_neighbour),
+  missed = missed_empty,
+  acc = 0,
+  augpath = None\<rparr>"
+(*
+definition "change_potential pot \<epsilon> even_verts odd_verts =
+            (foldl (\<lambda> pot v. add_to_pot pot v \<epsilon>) 
+               (foldl (\<lambda> pot v. add_to_pot pot v \<epsilon>) pot odd_verts)
+             even_verts)"
+*)
+function (domintros) search_path::
+  " ('forest, 'ben, 'heap, 'miss, 'v) hungarian_search_state \<Rightarrow>
+   ('forest, 'ben, 'heap, 'miss, 'v) hungarian_search_state" where
+"search_path state = 
+  (let F = forest state;
+       ben = best_even_neighbour state;
+       missed_\<epsilon> = missed_at state;
+       (queue, heap_min) = heap_extract_min (heap state)
+   in (case heap_min of
+          None \<Rightarrow> state \<lparr>augpath:=None\<rparr> |
+          Some r \<Rightarrow>
+            (let l = the (ben_lookup ben r);
+                 acc' = w\<^sub>\<pi> l r + missed_\<epsilon> l
+             in
+             (case buddy r of 
+                 None \<Rightarrow>
+                    state \<lparr> acc := acc',
+                            augpath:= Some (rev (get_path F l) @[r]) \<rparr>|
+                 Some l' \<Rightarrow>
+                     (let missed' = missed_upd (
+                                    missed_upd (missed state) r acc') 
+                                                l' acc';
+                          (ben', queue') = update_best_even_neighbour 
+                                           (abstract_real_map (missed_lookup missed'))
+                                           ben queue l';
+                          F'= extend_forest_even_unclassified F l r l' 
+                      in  
+                    search_path (state \<lparr> forest:= F', 
+                            best_even_neighbour:=ben',
+                            heap:=queue',
+                            missed:=missed',
+                            acc:= acc' \<rparr>)
+             )))))"
+  by pat_completeness auto
+
+definition "search_path_fail_cond state = 
+  (let (queue, heap_min) = heap_extract_min (heap state)
+   in (case heap_min of None \<Rightarrow> True|
+                        Some r \<Rightarrow> False))"
+
+lemma search_path_fail_condE:
+"search_path_fail_cond state \<Longrightarrow>
+(\<And> queue heap_min. 
+    \<lbrakk> (queue, heap_min) = heap_extract_min (heap state); heap_min = None\<rbrakk> \<Longrightarrow> P)
+\<Longrightarrow> P"
+  apply(cases "heap_extract_min (heap state)")
+  apply(all \<open>cases "snd (heap_extract_min (heap state))"\<close>)
+  by(auto simp add: search_path_fail_cond_def)
+
+definition "search_path_succ_cond state = 
+  (let (queue, heap_min) = heap_extract_min (heap state)
+   in (case heap_min of
+          None \<Rightarrow> False|
+          Some r \<Rightarrow> (case buddy r of 
+                        None \<Rightarrow> True|
+                        Some l' \<Rightarrow> False )))"
+
+lemma search_path_succ_condE:
+"search_path_succ_cond state \<Longrightarrow>
+(\<And> queue heap_min r. 
+    \<lbrakk> (queue, heap_min) = heap_extract_min (heap state); 
+        heap_min = Some r; buddy r = None\<rbrakk> \<Longrightarrow> P)
+\<Longrightarrow> P"
+  apply(cases "heap_extract_min (heap state)")
+  apply(all \<open>cases "snd (heap_extract_min (heap state))"\<close>)
+  apply(all \<open>cases "buddy (the (snd (heap_extract_min (heap state))))"\<close>)
+  by(auto simp add: search_path_succ_cond_def)
+
+definition "search_path_cont_cond state = 
+  (let (queue, heap_min) = heap_extract_min (heap state)
+   in (case heap_min of None \<Rightarrow> False|
+                        Some r \<Rightarrow> (case buddy r of None \<Rightarrow> False|
+                                                   Some l' \<Rightarrow> True)))"
+
+lemma search_path_cont_condE:
+"search_path_cont_cond state \<Longrightarrow>
+(\<And> queue heap_min r l'. 
+    \<lbrakk>  heap_extract_min (heap state) = (queue, heap_min); 
+        heap_min = Some r; buddy r = Some l'\<rbrakk> \<Longrightarrow> P)
+\<Longrightarrow> P"
+  apply(cases "heap_extract_min (heap state)")
+  apply(all \<open>cases "snd (heap_extract_min (heap state))"\<close>)
+  apply(all \<open>cases "buddy (the (snd (heap_extract_min (heap state))))"\<close>)
+  by(auto simp add: search_path_cont_cond_def)
+
+lemma search_path_cases:
+  assumes "search_path_fail_cond state \<Longrightarrow> P"
+          "search_path_succ_cond state \<Longrightarrow> P"
+          "search_path_cont_cond state \<Longrightarrow> P"
+    shows P
+  using assms
+  apply(cases "heap_extract_min (heap state)")
+  apply(all \<open>cases "snd (heap_extract_min (heap state))"\<close>)
+  apply(all \<open>cases "buddy (the (snd (heap_extract_min (heap state))))"\<close>)
+  by(auto simp add: search_path_fail_cond_def
+                    search_path_succ_cond_def search_path_cont_cond_def)
+
+definition "search_path_fail_upd state = state \<lparr>augpath:=None\<rparr>"
+
+definition "search_path_succ_upd state = 
+  (let F = forest state;
+       ben = best_even_neighbour state;
+       missed_\<epsilon> = missed_at state;
+       (queue, heap_min) = heap_extract_min (heap state);
+       r = the heap_min;
+       l = the (ben_lookup ben r);
+       acc' = w\<^sub>\<pi> l r + missed_\<epsilon> l
+    in state \<lparr> acc := acc', augpath:= Some (rev (get_path F l) @[r]) \<rparr>)"
+
+definition "search_path_cont_upd state = 
+  (let F = forest state;
+       ben = best_even_neighbour state;
+       missed_\<epsilon> = missed_at state;
+       (queue, heap_min) = heap_extract_min (heap state);
+       r = the heap_min;
+       l = the (ben_lookup ben r);
+        acc' = w\<^sub>\<pi> l r + missed_\<epsilon> l;
+       l' =  the (buddy r);
+       missed' = missed_upd (missed_upd (missed state) r acc') 
+                                                l' acc';
+       (ben', queue') = update_best_even_neighbour 
+                 (abstract_real_map (missed_lookup missed'))ben queue l';
+       F'= extend_forest_even_unclassified F l r l' 
+    in state \<lparr> forest:= F', best_even_neighbour:=ben',
+              heap:=queue', missed:=missed', acc:= acc' \<rparr>)"
+ 
+lemma search_path_simps:
+  "search_path_fail_cond state \<Longrightarrow> search_path state = search_path_fail_upd state"
+  "search_path_succ_cond state \<Longrightarrow> search_path state = search_path_succ_upd state"
+  "\<lbrakk>search_path_dom state; search_path_cont_cond state\<rbrakk> \<Longrightarrow>
+   search_path state = search_path (search_path_cont_upd state)"
+proof(goal_cases)
+  case 1
+  show ?case 
+    apply(subst search_path.psimps)
+    apply(all \<open>cases "heap_extract_min (heap state)"\<close>)
+    apply(all \<open>cases "snd (heap_extract_min (heap state))"\<close>)
+    using 1
+    by(auto intro: search_path.domintros
+             simp add: search_path_fail_cond_def search_path_fail_upd_def)
+next
+  case 2
+  show ?case
+    apply(subst search_path.psimps)
+    apply(all \<open>cases "heap_extract_min (heap state)"\<close>)
+    apply(all \<open>cases "snd (heap_extract_min (heap state))"\<close>)
+    apply(all \<open>cases "buddy (the (snd (heap_extract_min (heap state))))"\<close>)
+    using 2
+    by(auto intro: search_path.domintros
+             simp add: search_path_succ_cond_def search_path_succ_upd_def)
+next
+  case 3
+  show ?case 
+    apply(subst search_path.psimps[OF 3(1)])
+    apply(all \<open>cases "heap_extract_min (heap state)"\<close>)
+    apply(all \<open>cases "snd (heap_extract_min (heap state))"\<close>)
+    apply(all \<open>cases "buddy (the (snd (heap_extract_min (heap state))))"\<close>)
+    using 3
+    by(auto simp add: search_path_cont_cond_def search_path_cont_upd_def Let_def
+               split: option.split prod.split)
+qed
+
+lemma search_path_induct:
+  assumes "search_path_dom state"
+           "\<And> state. \<lbrakk>search_path_dom state;
+                      search_path_cont_cond state \<Longrightarrow> P (search_path_cont_upd state)\<rbrakk>
+                     \<Longrightarrow> P state"
+  shows "P state"
+proof(induction rule: search_path.pinduct[OF assms(1)])
+  case (1 state)
+  note IH = this
+  show ?case 
+  proof(cases state rule: search_path_cases, goal_cases)
+    case 1
+    then show ?case
+     by(auto elim!:  search_path_fail_condE
+            intro!: assms(2)[OF IH(1)]
+          simp add: search_path_cont_cond_def)
+  next
+    case 2
+    then show ?case 
+     by(auto elim!:  search_path_succ_condE
+            intro!: assms(2)[OF IH(1)] 
+          simp add: search_path_cont_cond_def)
+  next
+    case 3
+    show ?case 
+      apply(rule assms(2)[OF IH(1)])
+      using 3 assms(2)
+      by(auto intro!: IH(2)
+               elim!: search_path_cont_condE
+            simp add: search_path_cont_upd_def Let_def 
+               split: option.split prod.split)
+  qed
+qed
+
+partial_function (tailrec) search_path_impl::
+  " ('forest, 'ben, 'heap, 'miss, 'v) hungarian_search_state \<Rightarrow>
+   ('forest, 'ben, 'heap, 'miss, 'v) hungarian_search_state" where
+"search_path_impl state = 
+  (let F = forest state;
+       ben = best_even_neighbour state;
+       missed_\<epsilon> = missed_at state;
+       (queue, heap_min) = heap_extract_min (heap state)
+   in (case heap_min of
+          None \<Rightarrow> state \<lparr>augpath:=None\<rparr> |
+          Some r \<Rightarrow>
+            (let l = the (ben_lookup ben r);
+                 acc' = w\<^sub>\<pi> l r + missed_\<epsilon> l
+             in
+             (case buddy r of 
+                 None \<Rightarrow>
+                    state \<lparr> acc := acc',
+                            augpath:= Some (rev (get_path F l) @[r]) \<rparr>|
+                 Some l' \<Rightarrow>
+                     (let missed' = missed_upd (
+                                    missed_upd (missed state) r acc') 
+                                                l' acc';
+                          (ben', queue') = update_best_even_neighbour 
+                                           (abstract_real_map (missed_lookup missed'))
+                                           ben queue l';
+                          F'= extend_forest_even_unclassified F l r l' 
+                      in  
+            search_path_impl (state \<lparr> forest:= F', 
+                            best_even_neighbour:=ben',
+                            heap:=queue',
+                            missed:=missed',
+                            acc:= acc' \<rparr>)
+             )))))"
+
+lemma search_path_impl_same:
+  assumes "search_path_dom state"
+  shows "search_path_impl state = search_path state"
+  apply(induction rule: search_path.pinduct[OF assms])
+  apply(subst search_path.psimps, simp)
+  apply(subst search_path_impl.simps)
+  by (auto simp add: Let_def split: if_split option.split prod.split)
+
+definition "forest_extension_precond F M x y z =
+      (forest_invar M F \<and> x \<in> vset_to_set (evens F) \<and>
+        {y, z} \<inter> (vset_to_set (evens F) \<union> vset_to_set (odds F)) = {} \<and>
+        {x, y} \<notin> M \<and> {y, z} \<in> M)"
+
+lemma forest_extension_precondI:
+"\<lbrakk>forest_invar M F; x \<in> vset_to_set (evens F);
+  {y, z} \<inter> (vset_to_set (evens F) \<union> vset_to_set (odds F)) = {};
+  {x, y} \<notin> M; {y, z} \<in> M\<rbrakk>
+\<Longrightarrow>forest_extension_precond F M x y z "
+  by(auto simp add: forest_extension_precond_def)
+end
+
+
+locale primal_dual_path_search =
+        primal_dual_path_search_spec 
+      where G = "G::'v set set" 
+      and   left = "left::'vset"
+      and empty_forest="empty_forest::'vset \<Rightarrow> 'forest"
+      and initial_pot = "initial_pot::'pot"
+      and ben_empty="ben_empty::'ben"
+    for G left empty_forest initial_pot ben_empty
++
+assumes G: "bipartite G L R"
+           "\<And> u v. in_G u v \<longleftrightarrow> {u, v} \<in> G"
+           "vset_invar left" "vset_invar right"
+           "\<And> v. v \<in> vset_to_set left \<Longrightarrow> vset_invar (right_neighbs v)"
+           "\<And> v. v \<in> vset_to_set left \<Longrightarrow> vset_to_set (right_neighbs v) = {u | u. {v, u} \<in> G}"
+           "\<And> u v. {u, v} \<in> G \<Longrightarrow> edge_costs u v = edge_costs v u"
+           "\<And> u v. {u, v} \<in> G \<Longrightarrow> \<pi> u + \<pi> v \<le> \<w> u v"
+and matching: "\<And> u v. buddy u = Some v \<Longrightarrow> buddy v = Some u"
+              "graph_matching G {{u, v} | u v. buddy u = Some v}"
+              "\<And> u v. {u, v} \<in> \<M> \<Longrightarrow> \<pi> u + \<pi> v = \<w> u v"
+and forest_extend: "\<And> F M x y z. forest_extension_precond F M x y z
+      \<Longrightarrow> forest_invar M (extend_forest_even_unclassified F x y z)"
+   "\<And> F M x y z. forest_extension_precond F M x y z
+      \<Longrightarrow> abstract_forest (extend_forest_even_unclassified F x y z) =
+          abstract_forest F \<union> {{x, y}, {y, z}}"
+   "\<And> F M x y z. forest_extension_precond F M x y z
+      \<Longrightarrow> vset_to_set (evens (extend_forest_even_unclassified F x y z)) =
+          insert z (vset_to_set (evens F))"
+   "\<And> F M x y z. forest_extension_precond F M x y z
+      \<Longrightarrow> vset_to_set (odds (extend_forest_even_unclassified F x y z)) =
+          insert y (vset_to_set (odds F))"
+   "\<And> F M x y z. forest_extension_precond F M x y z
+      \<Longrightarrow> vset_to_set (roots (extend_forest_even_unclassified F x y z)) =
+          vset_to_set (roots F)"
+and evens_and_odds:
+ "\<And> F M. forest_invar M F\<Longrightarrow> vset_invar (evens F)"
+ "\<And> F M. forest_invar M F\<Longrightarrow> vset_invar (odds F)"
+ "\<And> F M. forest_invar M F
+      \<Longrightarrow> vset_to_set (evens F) \<union> vset_to_set (odds F) = 
+          vset_to_set (roots F) \<union> Vs (abstract_forest F)"
+  "\<And> F M. forest_invar M F\<Longrightarrow> 
+       (vset_to_set (evens F))\<inter>(vset_to_set (odds F)) = {}"
+and finite_forest:
+ "\<And> F M. forest_invar M F\<Longrightarrow> finite (vset_to_set (evens F))"
+ "\<And> F M. forest_invar M F\<Longrightarrow> finite (vset_to_set (odds F))"
+ "\<And> F M. forest_invar M F\<Longrightarrow> finite (abstract_forest F)"
+and roots:
+   "\<And> F M. forest_invar M F \<Longrightarrow> vset_invar (roots F)" 
+   "\<And> F M. forest_invar M F \<Longrightarrow> vset_to_set (roots F) \<subseteq> vset_to_set (evens F)" 
+and empty_forest:
+    "\<And> R. evens (empty_forest R) = R"
+    "\<And> R. odds (empty_forest R) = vset_empty"
+    "\<And> R. abstract_forest (empty_forest R) = {}"
+    "\<And> R. \<lbrakk>matching M; vset_invar R; vset_to_set R \<inter> Vs M = {}; 
+           finite (vset_to_set R); vset_to_set R \<noteq> {}\<rbrakk>
+          \<Longrightarrow> forest_invar M (empty_forest R)"
+and get_path:
+    "\<And> F M v p. \<lbrakk>forest_invar M F; v \<in> vset_to_set (evens F); p = get_path F v\<rbrakk> \<Longrightarrow>
+           alt_path M (rev p) \<and> odd (length p) \<and>
+           last p \<in> vset_to_set (roots F) \<and>
+           walk_betw (abstract_forest F) v p (last p)"
+and higher_forest_properties:
+    "\<And> F M. forest_invar M F\<Longrightarrow> 
+       card (vset_to_set (evens F)) > card (vset_to_set (odds F))"
+    "\<And> F M u v. \<lbrakk>forest_invar M F; {u, v} \<in> M\<rbrakk>\<Longrightarrow>
+        {u, v} \<in> abstract_forest F \<or> 
+          {u, v} \<inter> (Vs (abstract_forest F) \<union> vset_to_set (roots F)) = {}"
+    "\<And> F M u v. \<lbrakk>forest_invar M F; {u, v} \<in> abstract_forest F\<rbrakk>\<Longrightarrow>
+               u \<in> vset_to_set (evens F) \<longleftrightarrow> v \<in> vset_to_set (odds F)"
+and potential:
+ "potential_invar initial_pot"
+ "\<And> pot x s. potential_invar pot \<Longrightarrow> potential_invar (potential_upd pot x s)"
+ "\<And> pot x s. potential_invar pot \<Longrightarrow> potential_lookup (potential_upd pot x s) =
+                (potential_lookup pot)(x \<mapsto> s)"
+and best_even_neighbour:
+ "ben_invar ben_empty"
+  "\<And> ben x s. ben_invar ben \<Longrightarrow> ben_invar (ben_upd ben x s)"
+  "\<And> ben x s. ben_invar ben \<Longrightarrow> ben_lookup (ben_upd ben x s) =
+                (ben_lookup ben)(x \<mapsto> s)"
+  "\<And> x. ben_lookup ben_empty x = None"
+and vset:
+ "vset_invar vset_empty" "vset_to_set vset_empty = {}"
+ "\<And> V v. vset_invar V \<Longrightarrow> vset_invar (vset_insert v V)"
+ "\<And> V v. vset_invar V \<Longrightarrow> vset_to_set (vset_insert v V) = insert v (vset_to_set V)"
+ "\<And> V v. vset_invar V \<Longrightarrow> vset_isin v V \<longleftrightarrow> v \<in> vset_to_set V"
+ "\<And> V vs. \<lbrakk>vset_invar V; to_list V = vs\<rbrakk> \<Longrightarrow> distinct vs"
+ "\<And> V vs. \<lbrakk>vset_invar V; to_list V = vs\<rbrakk> \<Longrightarrow> set vs = vset_to_set V"
+and heap:
+ "heap_invar heap_empty"
+ "\<And> H. heap_invar H \<Longrightarrow> heap_invar (fst (heap_extract_min H))"
+ "\<And> H x k. \<lbrakk>heap_invar H; \<nexists> k. (x, k) \<in> (heap_abstract H)\<rbrakk> 
+          \<Longrightarrow> heap_invar (heap_insert H x k)"
+ "\<And> H x k k'. \<lbrakk>heap_invar H; (x, k') \<in>  (heap_abstract H); k < k'\<rbrakk> 
+          \<Longrightarrow> heap_invar (heap_decrease_key H x k)"
+
+ "\<And> H x.  \<lbrakk>heap_invar H; Some x = snd (heap_extract_min H)\<rbrakk> \<Longrightarrow>
+           \<exists> k. ((x, k) \<in> heap_abstract H \<and> 
+                (\<forall> x' k'. (x', k') \<in> heap_abstract H \<longrightarrow> k \<le> k'))"
+ "\<And> H.  \<lbrakk>heap_invar H; None = snd (heap_extract_min H)\<rbrakk> \<Longrightarrow>
+            heap_abstract H = {}"
+ "\<And> H x k k'. \<lbrakk>heap_invar H; (x, k) \<in> heap_abstract H; (x, k') \<in> heap_abstract H\<rbrakk>
+                  \<Longrightarrow> k = k'"
+
+ "\<And> H x k.  \<lbrakk>heap_invar H; Some x = snd (heap_extract_min H); (x, k) \<in> heap_abstract H\<rbrakk> \<Longrightarrow>
+           heap_abstract (fst (heap_extract_min H)) =  heap_abstract H - {(x, k)}"
+ "\<And> H x k k'.  \<lbrakk>heap_invar H;  (x, k) \<in> heap_abstract H; k' < k\<rbrakk> \<Longrightarrow>
+           heap_abstract (heap_decrease_key H x k') =
+           heap_abstract H - {(x, k)} \<union> {(x, k')}"
+ "\<And> H x k.  \<lbrakk>heap_invar H; \<nexists> k. (x, k) \<in> heap_abstract H\<rbrakk> \<Longrightarrow>
+           heap_abstract (heap_insert H x k) = heap_abstract H  \<union> {(x, k)}"
+ "heap_abstract heap_empty = {}"
+and missed:
+ "missed_invar missed_empty" "\<And> x. missed_lookup missed_empty x= None"
+  "\<And> missed x s. missed_invar missed \<Longrightarrow> missed_invar (missed_upd missed x s)"
+  "\<And> missed x s. missed_invar missed \<Longrightarrow> missed_lookup (missed_upd missed x s) =
+                (missed_lookup missed)(x \<mapsto> s)"
+  "\<And> x. missed_lookup missed_empty x = None"
+begin
+
+lemma w\<^sub>\<pi>_symmetric: "{u, v} \<in> G \<Longrightarrow> w\<^sub>\<pi> u v = w\<^sub>\<pi> v u"
+  by(auto simp add: w\<^sub>\<pi>_def intro: G(7))
+
+lemma w\<^sub>\<pi>_non_neg: "{u, v} \<in> G \<Longrightarrow> w\<^sub>\<pi> u v \<ge> 0"
+  using G(8) w\<^sub>\<pi>_def by fastforce
+
+lemma update_best_even_neighbour_correct:
+  assumes "ben_invar ben" "heap_invar queue" "l \<in> L"
+          "\<And> r k. (r, k) \<in> heap_abstract queue \<longrightarrow>
+          (\<exists> l. ben_lookup ben r = Some l \<and> k = w\<^sub>\<pi> l r + off l)"
+          "\<And> r l'. ben_lookup ben r = Some l' \<and> (\<nexists> k. (r, k) \<in> heap_abstract queue) \<longrightarrow>
+             off l \<ge> w\<^sub>\<pi> l' r + off l'"
+          "(ben', queue') = update_best_even_neighbour off ben queue l"
+ shows "ben_invar ben'" (is ?thesis1) "heap_invar queue'" (is ?thesis2)
+       "\<And> r k.  (r, k) \<in> heap_abstract queue' \<Longrightarrow> 
+        \<exists> l. ben_lookup ben' r = Some l \<and> k = w\<^sub>\<pi> l r + off l"
+        "\<And> r l'. ben_lookup ben' r = Some l' \<and> (\<nexists> k. (r, k) \<in> heap_abstract queue') \<Longrightarrow>
+             off l \<ge> w\<^sub>\<pi> l' r + off l'"
+      "ben_lookup ben' = (\<lambda> r. if r \<notin> vset_to_set (right_neighbs l) then ben_lookup ben r
+                               else if ben_lookup ben r = None 
+                                    then Some l
+                               else if w\<^sub>\<pi> l r + off l < 
+                                      w\<^sub>\<pi> (the (ben_lookup ben r)) r + off (the (ben_lookup ben r))
+                                    then Some l
+                                else ben_lookup ben r)" (is ?thesis3)
+      "heap_abstract queue' = 
+       heap_abstract queue
+       - {(r, k) | r k. r \<in> vset_to_set (right_neighbs l)}
+       \<union> {(r, min (w\<^sub>\<pi> l r + off l) 
+                  (w\<^sub>\<pi> (the (ben_lookup ben r)) r + off (the (ben_lookup ben r))))
+          | r. r \<in> vset_to_set (right_neighbs l) \<and> r \<in> fst ` (heap_abstract queue)}
+       \<union> { (r, w\<^sub>\<pi> l r + off l) 
+          | r . r \<in> vset_to_set (right_neighbs l) \<and> ben_lookup ben r = None}" (is ?thesis4)
+proof-
+  define f where "f = (\<lambda> (ben, queue) r.
+     case ben_lookup ben r of
+     None \<Rightarrow> (ben_upd ben r l, heap_insert queue r (w\<^sub>\<pi> l r + off l))
+     | Some l' \<Rightarrow>
+         if w\<^sub>\<pi> l r + off l < w\<^sub>\<pi> l' r + off l'
+         then (ben_upd ben r l, heap_decrease_key queue r (w\<^sub>\<pi> l r + off l))
+         else (ben, queue))"
+  define rs where "rs = rev (to_list (right_neighbs l))"
+  have rs_props: "distinct rs" "set rs = vset_to_set (right_neighbs l)"
+    using vset(6)[of "right_neighbs l"] G(5) assms(3)
+          vset(7)[of "right_neighbs l", OF _ refl]
+    by (auto simp add: rs_def)
+  have news_in_G:"{{l, r} | r. r \<in> set rs} \<subseteq> G" 
+    unfolding rs_props G(6)[OF assms(3)] by blast
+  have induction:"?thesis1 \<and> ?thesis2 \<and>
+        (\<forall> r k.  (r, k) \<in> heap_abstract queue' \<longrightarrow> 
+               (\<exists> l. ben_lookup ben' r = Some l \<and> k = w\<^sub>\<pi> l r + off l)) \<and>
+        (\<forall> r l'. ben_lookup ben' r = Some l' \<and> (\<nexists> k. (r, k) \<in> heap_abstract queue') \<longrightarrow>
+             off l \<ge> w\<^sub>\<pi> l' r + off l')
+           \<and> ?thesis3 \<and> ?thesis4"
+    using assms(1,2,4,5,6) rs_props(1)  news_in_G
+    unfolding update_best_even_neighbour_def foldl_conv_foldr
+    unfolding rs_def[symmetric] rs_props(2)[symmetric] f_def[symmetric]
+  proof(induction rs arbitrary: queue ben queue' ben')
+    case Nil
+    thus ?case
+      by simp
+  next
+    case (Cons r rs)
+    define ben_before where "ben_before = (fst (foldr (\<lambda>x y. f y x) rs (ben, queue)))"
+    define queue_before where "queue_before = (snd (foldr (\<lambda>x y. f y x) rs (ben, queue)))"
+    have state_before_is: "(ben_before, queue_before) = foldr (\<lambda>x y. f y x) rs (ben, queue)"
+      by(simp add: ben_before_def queue_before_def)
+    have ben'_is: "ben' = (fst (f (ben_before, queue_before) r))"
+                  "queue' = (snd (f (ben_before, queue_before) r))"
+      using Cons.prems(5) 
+      by (simp add: split_pairs ben_before_def queue_before_def)+
+    have distinct_rs: "distinct rs" using Cons(7) by auto
+  have news_in_G:"{{l, r} | r. r \<in> set rs} \<subseteq> G"
+    using Cons.prems(7) by auto
+  have pos_new_e:" w\<^sub>\<pi> l r \<ge> 0" 
+          using Cons.prems(7) w\<^sub>\<pi>_non_neg[of l r] by auto
+    note IH_applied_all = Cons(1)[OF Cons(2,3,4,5) state_before_is 
+             distinct_rs news_in_G]
+    note IH_applied = conjD(1)[OF IH_applied_all]
+                      conjD(2)[OF IH_applied_all]
+                      mp[OF spec[OF spec[OF conjD(3)[OF IH_applied_all]]]]
+                      mp[OF spec[OF spec[OF conjD(4)[OF IH_applied_all]]]]
+                      conjD(5)[OF IH_applied_all]
+                       conjD(6)[OF IH_applied_all]
+    show ?case 
+      unfolding ben'_is
+    proof(rule conj_intro, goal_cases)
+      case 1
+      then show ?case
+        using IH_applied
+        by(auto split: option.split 
+               intro!: best_even_neighbour(2) 
+             simp add: f_def)
+    next
+      case 2
+      have helper: "ben_lookup ben r = Some x2 \<Longrightarrow>
+          w\<^sub>\<pi> l r + off l < w\<^sub>\<pi> x2 r + off x2 \<Longrightarrow>
+          (r, w\<^sub>\<pi> x2 r + off x2) \<in> heap_abstract queue_before" for x2
+      proof(rule ccontr, goal_cases)
+        case 1
+        hence "(r, k) \<in> heap_abstract queue_before \<Longrightarrow> False" for k
+          using Cons.prems(6) IH_applied(3)[of r k] IH_applied(5) by simp
+        hence "\<nexists> k. (r, k) \<in> heap_abstract queue_before" by auto
+        hence "off l \<ge> w\<^sub>\<pi> x2 r + off x2"
+          using "1"(1) Cons.prems(6) IH_applied_all by auto
+        thus ?case
+          using "1"(2) pos_new_e by simp
+      qed
+      from 2 show ?case 
+        using IH_applied(1,2) IH_applied(3) Cons.prems(3)[of r] IH_applied(4)[of r]
+        by(auto split: option.split 
+               intro!: heap(3,4) helper 
+                 dest: IH_applied(3)
+             simp add: f_def IH_applied(5))
+    next
+      case 3
+      then show ?case
+      proof(cases "ben_lookup ben_before r")
+        case None
+        hence not_in_heap_before:"\<nexists>k. (r, k) \<in> heap_abstract queue_before" 
+          using IH_applied(3) by force
+        show ?thesis 
+        using IH_applied(1,2,3) not_in_heap_before
+        by(auto simp add: f_def best_even_neighbour(3) None 
+                          heap(10)[OF IH_applied(2) not_in_heap_before])
+      next
+        case (Some l')
+        hence in_heap_before: "w\<^sub>\<pi> l r + off l < w\<^sub>\<pi> l' r + off l' \<Longrightarrow> 
+            (r, w\<^sub>\<pi> l' r + off l') \<in> heap_abstract queue_before"
+          using IH_applied(4)[of r l'] IH_applied(3)[of r] pos_new_e by force
+        show ?thesis 
+        using IH_applied(1,2,3) heap(9,7)[OF IH_applied(2) in_heap_before]
+        by(auto simp add: f_def best_even_neighbour(3) Some)
+    qed
+    next
+      case 4
+      then show ?case 
+      proof(cases "ben_lookup ben_before r")
+        case None
+        hence not_in_heap_before:"\<nexists>k. (r, k) \<in> heap_abstract queue_before" 
+          using IH_applied(3) by force
+        show ?thesis 
+        using IH_applied(1,2)
+        by(auto simp add: f_def best_even_neighbour(3) None 
+                          heap(10)[OF IH_applied(2) not_in_heap_before] 
+                  intro!: IH_applied(4))
+      next
+        case (Some l')
+        hence in_heap_before: "w\<^sub>\<pi> l r + off l < w\<^sub>\<pi> l' r + off l' 
+              \<Longrightarrow>  (r, w\<^sub>\<pi> l' r + off l') \<in> heap_abstract queue_before"
+         using IH_applied(4)[of r l'] IH_applied(3)[of r] pos_new_e by force
+        show ?thesis 
+        using IH_applied(1,2,3)
+        by(auto simp add: f_def best_even_neighbour(3) Some
+                          heap(9)[OF IH_applied(2) in_heap_before]
+                  intro!: IH_applied(4))
+     qed
+    next
+      case 5
+      show ?case
+      proof(cases "ben_lookup ben_before r")
+        case None
+        hence not_in_heap_before:"\<nexists>k. (r, k) \<in> heap_abstract queue_before" 
+          using IH_applied(3) by force
+        show ?thesis 
+        using IH_applied(1,2)
+        by(auto simp add: f_def best_even_neighbour(3) None IH_applied(5))
+      next
+        case (Some l')
+        hence in_heap_before: "w\<^sub>\<pi> l r + off l < w\<^sub>\<pi> l' r + off l' 
+             \<Longrightarrow> (r, w\<^sub>\<pi> l' r + off l') \<in> heap_abstract queue_before"
+          using IH_applied(4)[of r l'] IH_applied(3)[of r] pos_new_e by force
+        show ?thesis 
+        using IH_applied(1,2,3)
+        by(auto simp add: f_def best_even_neighbour(3) Some IH_applied(5)
+                          heap(9)[OF IH_applied(2) in_heap_before])
+    qed
+  next
+    case 6
+     have ben_before_r_is:"ben_lookup ben_before r = ben_lookup ben r"
+          using Cons.prems(6) IH_applied(5) by auto
+    have Collect_Cons: "{f x | x. x \<in> set (y#ys)}
+              = insert ( f y) {f x | x. x \<in> set ys}"
+          for f y ys by auto
+      show ?case
+      proof(cases "ben_lookup ben_before r")
+        case None
+        hence not_in_heap_before:"\<nexists>k. (r, k) \<in> heap_abstract queue_before" 
+          using IH_applied(3) by force
+        show ?thesis 
+          unfolding Collect_Cons
+          using None ben_before_r_is Cons.prems(3)[of r]
+          by (auto simp add: f_def  None  IH_applied(6) 
+                             heap(10)[OF IH_applied(2) not_in_heap_before] )
+      next
+        case (Some l')
+        hence in_heap_before: 
+        "w\<^sub>\<pi> l r + off l < w\<^sub>\<pi> l' r + off l' \<Longrightarrow> (r, w\<^sub>\<pi> l' r + off l') \<in> heap_abstract queue_before"
+          using IH_applied(4)[of r l'] IH_applied(3)[of r] pos_new_e by force
+        have if_not_P2:"ben_lookup ben r \<noteq> None"
+          using Some ben_before_r_is by auto
+        have ben_of_r_is_l':"(the (ben_lookup ben r)) = l'" 
+          using Some ben_before_r_is by auto
+        have helper1: " (r, k) \<in> heap_abstract queue \<Longrightarrow> k = w\<^sub>\<pi> l' r + off l'" for k
+            using Some ben_before_r_is Cons.prems(3)[of r] Cons.prems(2,4)
+            by(auto intro: heap(7))
+        show ?thesis
+          unfolding Collect_Cons f_def split Some option.case(2)
+        proof(cases "w\<^sub>\<pi> l r + off l < w\<^sub>\<pi> l' r + off l'", goal_cases)
+          case 1
+          have helpers2: "(r, w\<^sub>\<pi> l r + off l) \<in> heap_abstract queue" False
+            if "w\<^sub>\<pi> l r + off l < w\<^sub>\<pi> l' r + off l'" "r \<notin> fst ` heap_abstract queue"
+               "ben_lookup ben r = Some l'"
+            using that Cons.prems(4) image_iff pos_new_e helper1 by fastforce+
+          have helpers3: "k = w\<^sub>\<pi> (the (ben_lookup ben r)) r + off (the (ben_lookup ben r))"
+            if "l' = the (ben_lookup ben r)" "(r, k) \<in> heap_abstract queue" for k
+            using that  Cons.prems(4) image_iff pos_new_e helper1 by fastforce
+          have helpers4: " k = w\<^sub>\<pi> l' r + off l'"
+            if"(r, k) \<in> heap_abstract queue" for k
+          using that  Cons.prems(4) image_iff pos_new_e helper1 by fastforce
+        from 1 show ?case 
+            unfolding if_P[OF 1] snd_conv if_not_P[OF if_not_P2] ben_of_r_is_l'
+                      heap(9)[OF IH_applied(2) in_heap_before[OF 1] 1]   
+                      IH_applied(6)
+            using  ben_of_r_is_l' helpers2 helpers3 helpers4 by auto
+        next
+          case 2
+          thus ?case
+            using Cons.prems(3,4,7) helper1 if_not_P2 Some ben_before_r_is
+            unfolding if_not_P[OF 2] snd_conv if_not_P[OF if_not_P2] ben_of_r_is_l'
+                      IH_applied(6)
+            by (auto simp add: rev_image_eqI)
+        qed
+      qed
+    qed
+  qed
+  show ?thesis1 ?thesis2
+    using conjD(1,2)[OF induction]
+    by simp+
+  show ?thesis3 
+    using conjD(5)[OF induction] by simp
+  show ?thesis4
+    using conjD(6)[OF induction] by simp
+  show"\<And> r k. (r, k) \<in> heap_abstract queue'
+         \<Longrightarrow> \<exists>l. ben_lookup ben' r = Some l \<and> k = w\<^sub>\<pi> l r + off l"
+    using conjD(3)[OF induction] by auto
+  show "\<And> r l'. ben_lookup ben' r = Some l' \<and> (\<nexists>k. (r, k) \<in> heap_abstract queue') \<Longrightarrow>
+        w\<^sub>\<pi> l' r + off l' \<le> off l"
+    using conjD(4)[OF induction] by auto
+qed
+
+lemma update_best_even_neighbours_correct:
+  assumes "ben_invar ben" "heap_invar queue" "set ls \<subseteq> L"
+          "\<And> r k. (r, k) \<in> heap_abstract queue \<longrightarrow>
+          (\<exists> l. ben_lookup ben r = Some l \<and> k = w\<^sub>\<pi> l r + off l)"
+          "\<And> r l' l. ben_lookup ben r = Some l' \<and> (\<nexists> k. (r, k) \<in> heap_abstract queue)  \<longrightarrow>
+             off l \<ge> w\<^sub>\<pi> l' r + off l'"
+          "(ben', queue') = update_best_even_neighbour off ben queue l"
+ defines "conn_min \<equiv> (\<lambda> r.
+     Min ((if ben_lookup ben r \<noteq> None 
+          then {w\<^sub>\<pi> (the (ben_lookup ben r)) r + off (the (ben_lookup ben r))}
+          else {}) \<union> 
+          {w\<^sub>\<pi> l r + off l | l. l \<in> set ls \<and> r \<in> vset_to_set (right_neighbs l) }))"
+ shows "ben_invar ben'" (is ?thesis1) "heap_invar queue'" (is ?thesis2)
+       "\<And> r k. (r, k) \<in> heap_abstract queue' \<Longrightarrow>
+         (\<exists> l. ben_lookup ben' r = Some l \<and> k = w\<^sub>\<pi> l r + off l)"
+       "\<And> r l'. ben_lookup ben' r = Some l' \<and> (\<nexists> k. (r, k) \<in> heap_abstract queue) \<Longrightarrow>
+             off l \<ge> w\<^sub>\<pi> l' r + off l'"
+       "\<And> r. r \<notin> \<Union> {vset_to_set (right_neighbs l)| l. l \<in> set ls} 
+                 \<Longrightarrow> ben_lookup ben' r = ben_lookup ben r"
+       "\<And> r. r \<in> \<Union> {vset_to_set (right_neighbs l)| l. l \<in> set ls} 
+                 \<Longrightarrow> \<exists> l. ((l \<in> set ls \<and> r \<in> vset_to_set (right_neighbs l))
+                            \<or> Some l = ben_lookup ben r) 
+                          \<and> w\<^sub>\<pi> l r + off l = conn_min r \<and> ben_lookup ben' r = Some l"
+      "heap_abstract queue' = 
+       heap_abstract queue
+           - {(r, k) | r k l. r \<in> vset_to_set (right_neighbs l) \<and>l \<in> set ls}
+           \<union> {(r, w\<^sub>\<pi> ll r + off ll) | r l ll. r \<in> vset_to_set (right_neighbs l) \<and> 
+                                         l \<in> set ls \<and> Some ll = ben_lookup ben' r}"
+               (is ?thesis4)
+proof-
+  define ls' where "ls' = rev ls"
+  have set_ls_is:"set ls = set ls'"
+    by(auto simp add: ls'_def)
+  have "?thesis1 \<and> ?thesis2 \<and>
+       (\<forall> r k. (r, k) \<in> heap_abstract queue' \<longrightarrow> 
+          (\<exists> l. ben_lookup ben' r = Some l \<and> k = w\<^sub>\<pi> l r + off l)) \<and>
+       (\<forall> r l. ben_lookup ben' r = Some l \<longrightarrow> (r, w\<^sub>\<pi> l r + off l) \<in> heap_abstract queue') \<and>
+       (\<forall> r.  r \<notin> \<Union> {vset_to_set (right_neighbs l)| l. l \<in> set ls} \<longrightarrow> 
+         ben_lookup ben' r = ben_lookup ben r) \<and>
+       (\<forall> r \<in> \<Union> {vset_to_set (right_neighbs l)| l. l \<in> set ls}.  
+         \<exists>l. ((l \<in> set ls \<and> r \<in> vset_to_set (right_neighbs l))
+                  \<or> Some l = ben_lookup ben r) \<and> 
+             w\<^sub>\<pi> l r + off l = conn_min r \<and> ben_lookup ben' r = Some l) \<and>
+       ?thesis4"
+    using assms(1-6) meta_eq_to_obj_eq[OF assms(7)]
+    unfolding update_best_even_neighbours_def foldl_conv_foldr
+              ls'_def[symmetric] set_ls_is
+  proof(induction ls' arbitrary: ben' queue' queue ben conn_min)
+    case (Cons l ls)
+    have ls_in_L: "set ls \<subseteq> L"
+      using Cons(4) by auto
+    define result where "result = 
+      foldr (\<lambda>x y. update_best_even_neighbour off (fst y) (snd y) x) ls (ben, queue)"
+    define ben_before where "ben_before = 
+     fst result"
+    define queue_before where "queue_before = 
+     snd result"
+    have result_is: "(fst result, snd result) = result"
+      by auto
+    define conn_min_before where "conn_min_before =
+       (\<lambda>r. Min ((if ben_lookup ben r \<noteq> None
+            then {w\<^sub>\<pi> (the (ben_lookup ben r)) r + off (the (ben_lookup ben r))}
+            else {}) \<union>
+           {w\<^sub>\<pi> l r + off l | l. (l \<in> set ls \<and> r \<in> vset_to_set (right_neighbs l))}))"
+
+    note IH_applied_all =
+       Cons(1)[OF Cons(2,3) ls_in_L Cons(5,6), simplified result_def[symmetric], 
+            OF result_is conn_min_before_def]
+    note IH_applied = conjD(1)[OF IH_applied_all]
+                      conjD(2)[OF IH_applied_all]
+                      spec[OF spec[OF conjD(3)[OF IH_applied_all]]]
+                      spec[OF spec[OF conjD(4)[OF IH_applied_all]]]
+                      conjD(5)[OF IH_applied_all]
+                      conjunct1[OF conjD(6)[OF IH_applied_all]]
+                      conjunct2[OF conjD(6)[OF IH_applied_all]]
+    thm Cons(7)
+    thm Cons(7)[simplified foldr_Cons o_apply]
+    have l_in_L: "l \<in> L" 
+      using Cons(4) by simp
+    have queue'_heap': "(ben', queue') = 
+          update_best_even_neighbour off (fst result) (snd result) l"
+      by(auto simp add: result_def Cons(7))
+    note single_update = update_best_even_neighbour_correct[OF
+            IH_applied(1,2) l_in_L IH_applied(3,4) queue'_heap']
+    show ?case 
+    proof(rule conj_intro, goal_cases)
+      case 1
+      then show ?case 
+        using single_update(1) by simp
+    next
+      case 2
+      then show ?case
+        using single_update(2) by simp
+    next
+      case 3
+      then show ?case 
+        using single_update(3) by simp
+    next
+      case 4
+      then show ?case 
+        using  single_update(4) by simp
+    next
+      case 5
+      then show ?case 
+        using IH_applied(5) single_update(5) by fastforce
+    next
+      case 6
+      show ?case 
+      proof(rule, rule ballI, goal_cases)
+        case (1 r)
+        note one = this
+        show ?case 
+          unfolding single_update(5) 
+        proof(cases "r \<notin> vset_to_set (right_neighbs l)", goal_cases)
+          case 1
+          hence old_conn_min: "conn_min r =  conn_min_before r"
+            by(auto intro: arg_cong[of _ _ Min] 
+                 simp add: Cons.prems(7) conn_min_before_def )
+          obtain l where l: "( (l \<in> set ls \<and> r \<in> vset_to_set (right_neighbs l)) \<or> Some l = ben_lookup ben r)"
+           "w\<^sub>\<pi> l r + off l = conn_min_before r \<and> ben_lookup (fst result) r = Some l"
+            using 1 one IH_applied(6) by auto
+          show ?case
+            using l 1
+            by(auto intro!: exI[of _ l] simp add:  old_conn_min)
+        next
+          case 2
+          note two = this
+          show ?case
+            unfolding if_not_P[OF 2]
+          proof(cases "ben_lookup (fst result) r", goal_cases)
+            case 1
+            hence r_not_previously:
+                "r \<notin> \<Union> {vset_to_set (right_neighbs l)| l. l \<in> set ls}"
+              using IH_applied_all by blast
+            hence init_None:"\<not> (ben_lookup ben r \<noteq> None)" 
+              using IH_applied(5)
+              using "1" by presburger 
+            show ?case
+              unfolding Cons.prems(7)  if_P[OF 1] if_not_P[OF init_None]
+              apply(rule exI[of _ l] )
+              apply(rule forw_subst[of _ "{w\<^sub>\<pi> l r + off l}"])
+              using  r_not_previously two
+              by auto
+          next
+            case (2 ll)
+            have "\<exists>l. ((l \<in> set ls \<and> r \<in> vset_to_set (right_neighbs l)) \<or> Some l = ben_lookup ben r) \<and>
+              w\<^sub>\<pi> l r + off l = conn_min_before r \<and> ben_lookup (fst result) r = Some l"
+              apply(cases "r \<in> \<Union> {vset_to_set (right_neighbs l)| l. l \<in> set ls}")
+              subgoal
+                using IH_applied(6) by auto
+              subgoal
+                apply(rule exI[of _ ll])
+                unfolding conn_min_before_def
+              apply(rule forw_subst[of _ "{w\<^sub>\<pi> ll r + off ll}"])
+              using  two IH_applied(5) 2
+              by(auto intro!:  exI[of _ "the (ben_lookup ben r)"])
+            done
+          hence ll_props: "((ll \<in> set ls \<and> r \<in> vset_to_set (right_neighbs ll)) \<or> Some ll = ben_lookup ben r)"
+              "w\<^sub>\<pi> ll r + off ll = conn_min_before r" 
+              "ben_lookup (fst result) r = Some ll"
+            using 2 by auto
+          have conn_min_is: "conn_min r = min (w\<^sub>\<pi> l r + off l) (conn_min_before r)"
+            using ll_props
+            unfolding Cons.prems(7) conn_min_before_def
+            apply(subst linorder_class.Min_insert[symmetric])
+              defer defer
+              apply(rule arg_cong[of _ _ Min])
+            using IH_applied(5) two by auto
+          show ?case
+            using 2 two ll_props(1)
+            by (auto simp add: "2" ll_props(1,2) conn_min_is)+
+        qed
+      qed
+      next
+        case 2
+        have queue'_is:"heap_abstract queue' =
+             heap_abstract (snd result) 
+               - {(r, k) | r k. r \<in> vset_to_set (right_neighbs l)} \<union>
+               {(r, w\<^sub>\<pi> ll r + off ll) | r ll. r \<in> vset_to_set (right_neighbs l) \<and>
+                     Some ll = ben_lookup ben' r}" 
+        proof(rule set_eqI, rule, goal_cases)
+          case (1 queue_entry)
+          then show ?case 
+          proof(cases  queue_entry, goal_cases)
+            case (1 r' k)
+            have helper: False if 
+               "\<And> ll. k = w\<^sub>\<pi> ll r' + off ll \<Longrightarrow> Some ll \<noteq> ben_lookup ben' r'"
+              "(r', k) =
+               (if ben_lookup (fst result) r = None then (r, w\<^sub>\<pi> l r + off l)
+                else if w\<^sub>\<pi> l r + off l
+                  < w\<^sub>\<pi> (the (ben_lookup (fst result) r)) r +
+                    off (the (ben_lookup (fst result) r))
+                   then (r, w\<^sub>\<pi> l r + off l)
+                   else (r, w\<^sub>\<pi> (the (ben_lookup (fst result) r)) r +
+                        off (the (ben_lookup (fst result) r))))"
+               "r' \<in> vset_to_set (right_neighbs l)" for r
+              using that
+              apply(cases "ben_lookup (fst result) r = None") 
+              apply( all \<open>cases "w\<^sub>\<pi> l r + off l
+                    < w\<^sub>\<pi> (the (ben_lookup (fst result) r)) r +
+                        off (the (ben_lookup (fst result) r))"\<close>)
+              by(force simp add: single_update(5))+
+            from 1 show ?thesis  
+             unfolding single_update(6) 
+             by auto (auto intro: helper simp add: single_update(5))
+         qed
+       qed (force simp add: single_update(5,6))       
+       show ?case 
+         unfolding  queue'_is  IH_applied(7)
+         unfolding Un_Diff  Un_assoc
+       proof(rule arg_cong2[where f = union], goal_cases)
+         case 2
+         have helper: "r \<in> vset_to_set (right_neighbs l)"
+           if "\<And> la lla. \<lbrakk>r \<in> vset_to_set (right_neighbs la);
+                              w\<^sub>\<pi> ll r + off ll = w\<^sub>\<pi> lla r + off lla\<rbrakk>\<Longrightarrow>
+                   la \<noteq> l \<and> la \<notin> set ls \<or> Some lla \<noteq> ben_lookup ben' r"
+             "r \<in> vset_to_set (right_neighbs la)" "la \<in> set ls"
+             " Some ll = ben_lookup (fst result) r" for r ll la
+             using that
+             by(cases "r \<notin> vset_to_set (right_neighbs l)") 
+               (auto simp add: single_update(5))
+           show ?case
+             using single_update(5) 
+             by (fastforce intro: helper)
+         qed auto
+       qed
+     qed
+   qed auto
+   thus  "\<And> r k. (r, k) \<in> heap_abstract queue' \<Longrightarrow> ben_lookup ben' r \<noteq> None" 
+        ?thesis1 ?thesis2 ?thesis4       
+        "\<And> r l. ben_lookup ben' r = Some l \<Longrightarrow> (r, w\<^sub>\<pi> l r + off l) \<in> heap_abstract queue'"
+        "\<And> r. r \<notin> \<Union> {vset_to_set (right_neighbs l)| l. l \<in> set ls} 
+                 \<Longrightarrow> ben_lookup ben' r = ben_lookup ben r"
+        "\<And> r. r \<in> \<Union> {vset_to_set (right_neighbs l)| l. l \<in> set ls} 
+                 \<Longrightarrow> \<exists> l. ((l \<in> set ls \<and> r \<in> vset_to_set (right_neighbs l))
+                             \<or> Some l = ben_lookup ben r) 
+                          \<and> w\<^sub>\<pi> l r + off l = conn_min r \<and> ben_lookup ben' r = Some l"
+    by (fast, auto)
+ qed
+(*TODO MOVE*)
+lemma matchingI:
+  "(\<And>e1 e2. \<lbrakk>e1 \<in> M; e2 \<in> M; e1 \<noteq> e2\<rbrakk> \<Longrightarrow> e1 \<inter> e2 = {}) \<Longrightarrow> matching M"
+  by (auto simp: matching_def)
+
+lemma \<M>_is_matching: "matching \<M>"
+proof(rule matchingI, rule ccontr, goal_cases)
+  case (1 e1 e2)
+  obtain u v where uv: "buddy u = Some v" "e1 ={u, v}"
+    using 1(1) by(force simp add: \<M>_def doubleton_eq_iff)
+  obtain u' v' where u'v': "buddy u' = Some v'" "e2 ={u', v'}"
+    using 1(2) by(force simp add: \<M>_def doubleton_eq_iff)
+  have more_buddies: "buddy v = Some u" "buddy v' =  Some u'"
+    using matching(1) uv(1) u'v'(1) by blast+
+  then show ?case 
+    using uv u'v' more_buddies 1(3,4)
+    by auto
+qed
+
+lemma one_buddy_no_buddy_false: 
+"\<lbrakk>Some v = buddy u;  None = buddy v\<rbrakk> \<Longrightarrow> False"
+  using  matching(1)[of u v] by simp
+
+lemma unmatched_lefts:
+ "set (unmatched_lefts) = L - Vs \<M>"
+ "length (unmatched_lefts) = card (L - Vs \<M>)"
+proof-
+  show  "set (unmatched_lefts) = L - Vs \<M>"
+  proof(rule, all \<open>rule\<close>, goal_cases)
+    case (1 x)
+    then show ?case 
+  using vset(6,7)[OF G(3) refl] 
+  by(cases "buddy x")
+    (auto elim!: vs_member_elim 
+      intro: one_buddy_no_buddy_false 
+      simp add: unmatched_lefts_def \<M>_def)
+  next
+    case (2 x)
+    then show ?case 
+    using vset(6,7)[OF G(3) refl] vs_member_intro[of "x" "{x, the (buddy x)}" \<M>]
+    by(cases "buddy x")
+      (fastforce intro: one_buddy_no_buddy_false 
+      simp add: unmatched_lefts_def \<M>_def doubleton_eq_iff)+ 
+qed
+  thus "length unmatched_lefts = card (L - Vs \<M>)"
+    using  distinct_card[of unmatched_lefts] distinct_filter[of unmatched_lefts]
+           vset(6)[OF G(3) refl]
+    by(auto simp add: unmatched_lefts_def) 
+qed  
+
+lemma unmatched_lefts_in_L: "set unmatched_lefts \<subseteq> L"
+  using unmatched_lefts by simp
+
+lemma to_list_left_is_L:"set (to_list left) = L"
+  using G(3) vset(7) by blast
+
+lemma M_verts_by_buddy:
+ "x \<in> Vs \<M> \<Longrightarrow> buddy x \<noteq> None"
+ "buddy x \<noteq> None \<Longrightarrow> x \<in> Vs \<M>"
+proof(goal_cases)
+  case 1
+  then show ?case  
+  using vset(6,7)[OF G(3) refl] 
+  by(cases "buddy x")
+    (auto elim!: vs_member_elim 
+      intro: one_buddy_no_buddy_false 
+      simp add: unmatched_lefts_def \<M>_def)
+next
+  case 2
+  then obtain y where "buddy x = Some y"
+    by auto
+  hence "{x, y} \<in> \<M>"
+    by(auto simp add: \<M>_def intro: exI[of _ x])
+  then show ?case 
+    by blast 
+qed
+
+lemma finite_G: "finite G" 
+  by (metis G(1,4) List.finite_set finite_parts_bipartite_graph_invar graph_invar_finite
+      to_list_left_is_L vset(7))
+
+context
+  assumes there_are_unmatched_lefts: "L -  Vs \<M> \<noteq> {}"
+begin
+
+lemma forest_roots:
+"vset_invar forest_roots"
+"vset_to_set forest_roots = L - Vs \<M>"
+"vset_to_set forest_roots \<noteq> {}"
+"finite (vset_to_set forest_roots)"
+"vset_to_set forest_roots \<inter> Vs \<M> = {}"
+proof-
+  define vs where "vs = rev unmatched_lefts"
+  have helper:
+      "vset_invar (foldl (\<lambda>vset v. vset_insert v vset) vset_empty unmatched_lefts) \<and>
+       vset_to_set (foldl (\<lambda>vset v. vset_insert v vset) vset_empty unmatched_lefts) = 
+       set unmatched_lefts"
+    unfolding foldl_conv_foldr vs_def[symmetric]
+              set_rev[of unmatched_lefts, symmetric]
+    by(induction vs)
+      (auto simp add: vset(1-4))
+  thus ths1and2:"vset_invar forest_roots" "vset_to_set forest_roots = L - Vs \<M>"
+    using   M_verts_by_buddy
+    by(force simp add: forest_roots_def unmatched_lefts_def 
+                       conjunct2[OF helper, simplified unmatched_lefts_def] 
+                       to_list_left_is_L[symmetric])+
+  thus "vset_to_set forest_roots \<noteq> {}"
+    using there_are_unmatched_lefts by auto
+  show "finite (vset_to_set forest_roots)" 
+    by (simp add: forest_roots_def helper)
+  show "vset_to_set forest_roots \<inter> Vs \<M> = {}" 
+    by (simp add: inf.commute ths1and2(2))
+qed
+
+lemmas props_of_init_heap_and_ben = 
+update_best_even_neighbours_correct[OF best_even_neighbour(1) heap(1)
+ unmatched_lefts_in_L, simplified best_even_neighbour heap(11),
+ of "\<lambda> x. 0", simplified, folded init_best_even_neighbour_def]
+
+lemma invars_init:
+"invar_basic initial_state"
+"invar_feasible_potential initial_state"
+"invar_forest_tight initial_state"
+"invar_matching_tight initial_state"
+"invar_best_even_neighbour_heap initial_state"
+"invar_best_even_neighbour_map initial_state"
+proof(goal_cases)
+  case 1
+    have helper:"dom (ben_lookup (best_even_neighbour initial_state)) =
+        {r | r l. r \<in> vset_to_set (right_neighbs l) \<and> l \<in> set unmatched_lefts}"
+    proof(rule set_eqI, goal_cases)
+      case (1 x)
+      then show ?case 
+      using  props_of_init_heap_and_ben(5,6)[OF surjective_pairing[symmetric], of x] 
+      by (auto simp add: initial_state_def)+
+     qed
+  show ?case 
+  proof(rule  invar_basicI, goal_cases)
+    case 1
+    then show ?case 
+    using forest_roots
+    by(auto intro!: empty_forest(4) 
+          simp add: initial_state_def  \<M>_is_matching) 
+  next
+    case 2
+    then show ?case  
+    by(simp add: initial_state_def 
+                 props_of_init_heap_and_ben(1,2)[OF surjective_pairing[symmetric]])     
+  next
+    case 3
+    then show ?case 
+    by(simp add: initial_state_def 
+                 props_of_init_heap_and_ben(1,2)[OF surjective_pairing[symmetric]])
+  next
+    case 4
+    then show ?case 
+      by (simp add: initial_state_def missed(1))
+  next
+    case 5
+    then show ?case 
+      by (simp add: empty_forest(3) initial_state_def)
+  next
+    case 6
+     show ?case 
+       using G(6) unmatched_lefts_in_L
+       by(auto simp add: helper)
+  next
+    case 7
+     show ?case 
+       by (simp add: domIff missed(2) primal_dual_path_search_spec.initial_state_def
+           subset_iff)
+  next
+    case 8
+    have helper:"fst ` heap_abstract (heap initial_state) =
+        {r | r l. r \<in> vset_to_set (right_neighbs l) \<and> l \<in> set unmatched_lefts}"
+    proof(rule, all \<open>rule\<close>, goal_cases)
+      case (1 x)
+      then show ?case 
+        by(auto simp add: initial_state_def
+            props_of_init_heap_and_ben(7)[OF surjective_pairing[symmetric]])
+    next
+      case (2 x)
+      then obtain l where l: "l \<in> set unmatched_lefts" "x \<in> vset_to_set (right_neighbs l)"
+        by blast
+       obtain l where l: "l \<in> set unmatched_lefts" "x \<in> vset_to_set (right_neighbs l)"
+              "ben_lookup (fst init_best_even_neighbour) x = Some l"
+         using props_of_init_heap_and_ben(6)[OF surjective_pairing[symmetric], of x] l
+                by blast
+        then show ?case
+            by(auto simp add: initial_state_def
+               props_of_init_heap_and_ben(7)[OF surjective_pairing[symmetric]]
+              intro!: image_eqI[of _ _ "(x, w\<^sub>\<pi> l x)"])
+        qed
+     show ?case 
+       using G(6) unmatched_lefts_in_L
+       by(auto simp add: helper)
+   next
+     case 9
+     show ?case
+       by(auto simp add: initial_state_def empty_forest(1) forest_roots(2))
+   next
+     case 10
+     show ?case
+       by (simp add: empty_forest(2) initial_state_def vset(2))
+   qed
+next
+  case 2
+  then show ?case 
+    using G(8)
+    by(auto intro!: invar_feasible_potentialI
+          simp add:  initial_state_def working_potential_def missed(2) 
+         abstract_real_map_def)
+next
+  case 3
+  then show ?case 
+    by(auto intro!: invar_forest_tightI
+          simp add:  initial_state_def empty_forest(3))
+next
+  case 4
+  then show ?case
+    using matching(3)
+    by(auto intro!: invar_matching_tightI
+          simp add:  initial_state_def empty_forest(3)
+                     working_potential_def empty_forest(1,2) missed(2)
+                     abstract_real_map_def)
+next
+  case 5
+  have help1: "(a, b) \<in> heap_abstract (snd init_best_even_neighbour) 
+                  \<Longrightarrow> a \<in> Vs G" for a b
+    by (auto intro: edges_are_Vs_2 
+          simp add: G(6)[OF set_mp[OF unmatched_lefts_in_L]]
+                    props_of_init_heap_and_ben(7)[OF surjective_pairing[symmetric]])
+  have help2: "\<lbrakk>(a, b) \<in> heap_abstract (snd init_best_even_neighbour);
+                a \<in> vset_to_set forest_roots\<rbrakk> \<Longrightarrow> False" for a b
+    by(auto simp add: props_of_init_heap_and_ben(7)[OF surjective_pairing[symmetric]]
+                      forest_roots(2) unmatched_lefts G(6) 
+                dest: bipartite_edgeD(1)[OF _ G(1)])
+  have help3: "(a, b) \<in> heap_abstract (snd init_best_even_neighbour) \<Longrightarrow>
+           \<exists>l. b = w\<^sub>\<pi> l a \<and> ben_lookup (fst init_best_even_neighbour) a = Some l"
+    for a b
+    by(auto simp add: props_of_init_heap_and_ben(7)[OF surjective_pairing[symmetric]]
+                      forest_roots(2) unmatched_lefts)
+  have help4:"(a, w\<^sub>\<pi> l a) \<in> heap_abstract (snd init_best_even_neighbour)" 
+    if "a \<in> Vs G" "a \<notin> vset_to_set forest_roots"
+       "ben_lookup (fst init_best_even_neighbour) a = Some l" for a l
+    using that
+          props_of_init_heap_and_ben(5)[OF surjective_pairing[symmetric], of a]
+    by(auto simp add: props_of_init_heap_and_ben(7)[OF surjective_pairing[symmetric]]
+                      forest_roots(2) unmatched_lefts)
+  show ?case 
+    by(auto intro!: help1 help2 help3 help4 invar_best_even_neighbour_heapI
+         simp add: initial_state_def missed(2) abstract_real_map_def
+                   empty_forest(1,2) vset(2))
+next
+  case 6
+  have helper1: False if
+        "r \<in> Vs G"" r \<notin> vset_to_set forest_roots"
+        "\<forall>l. l \<in> vset_to_set forest_roots \<longrightarrow> {l, r} \<notin> G"
+        "r \<in> vset_to_set (right_neighbs l)" "l \<in> set unmatched_lefts" for r l
+    using that by(simp add: G(6) forest_roots(2) unmatched_lefts(1))
+  have helper2: "\<exists>l. ben_lookup (fst init_best_even_neighbour) r = Some l \<and>
+               {r, l} \<in> G \<and> l \<in> vset_to_set forest_roots\<and>
+               w\<^sub>\<pi> l r =
+               Min {(w\<^sub>\<pi> l r) | l. l \<in> vset_to_set forest_roots \<and> {l, r} \<in> G}"
+    if  "r \<in> Vs G" "r \<notin> vset_to_set forest_roots"
+        "l \<in> vset_to_set forest_roots" "{l, r} \<in> G" for l r
+  proof-
+    have first_step:
+     "\<exists>x. (\<exists>l. x = vset_to_set (right_neighbs l) \<and> l \<in> set unmatched_lefts) \<and> r \<in> x"
+      using that unmatched_lefts(1) forest_roots(2)
+      by(auto intro!: exI[of _ "vset_to_set (right_neighbs l)"] exI[of _ l]
+             simp add:  G(6))
+    then obtain l' where l': "l' \<in> set unmatched_lefts"
+        "r \<in> vset_to_set (right_neighbs l')"
+        "w\<^sub>\<pi> l' r =
+        Min {w\<^sub>\<pi> l r | l. l \<in> set unmatched_lefts \<and> r \<in> vset_to_set (right_neighbs l)}"
+        "ben_lookup (fst init_best_even_neighbour) r = Some l'"
+      using props_of_init_heap_and_ben(6)[OF surjective_pairing[symmetric], of r] 
+      by auto     
+    then show ?thesis
+      using G(6) forest_roots(2) unmatched_lefts(1)
+      by (auto intro!: arg_cong[of _ _ Min] simp add: insert_commute)
+   qed
+   show ?case 
+     by(force intro: invar_best_even_neighbour_mapI helper1 helper2
+                     props_of_init_heap_and_ben(5)[OF surjective_pairing[symmetric]]
+         simp add: initial_state_def missed(2) abstract_real_map_def
+                   empty_forest(1,2) vset(2))
+ qed
+(*
+lemma assumes "invar_basic state"
+  shows "aevens state \<subseteq> L"
+proof(rule, goal_cases)
+  case (1 x)
+  have "odd (length (get_path (forest state) x))"
+       "last (get_path (forest state) x) \<in> vset_to_set (roots (forest state))"
+       "walk_betw (\<F> state) x (get_path (forest state) x) (last (get_path (forest state) x))"
+    using get_path[of \<M> "forest state" x, OF _ 1 refl] assms
+    by(auto elim: invar_basicE)
+  moreover hence "last (get_path (forest state) x) \<in> L"
+    using assms apply(auto elim!: invar_basicE)
+
+    
+  thm bipartite_even_and_odd_walk(1)
+  find_theorems bipartite 
+  then show ?case 
+    find_theorems evens get_path
+next
+  case 2
+  then show ?case sorry
+qed
+*)
+lemma invar_pres_one_step:
+  assumes "search_path_cont_cond state"
+          "invar_basic state"
+          "invar_feasible_potential state"
+          "invar_forest_tight state"
+          "invar_matching_tight state"
+          "invar_best_even_neighbour_heap state"
+          "invar_best_even_neighbour_map state"
+    shows "invar_basic (search_path_cont_upd state)"
+          "invar_feasible_potential (search_path_cont_upd state)"
+          "invar_forest_tight (search_path_cont_upd state)"
+          "invar_matching_tight (search_path_cont_upd state)"
+          "invar_best_even_neighbour_heap (search_path_cont_upd state)"
+          "invar_best_even_neighbour_map (search_path_cont_upd state)"
+proof-
+define F where "F = forest state"
+define ben where "ben = best_even_neighbour state"
+  define missed_\<epsilon> where  "missed_\<epsilon> = missed_at state"
+  obtain queue heap_min where queue_heap_min_def:
+      " (queue, heap_min) = heap_extract_min (heap state)"
+    by(cases "heap_extract_min (heap state)") auto
+  obtain r where r_def: "heap_min = Some r"
+   using queue_heap_min_def assms(1)
+   by(auto elim: search_path_cont_condE)
+  define l where "l = the (ben_lookup ben r)"
+  define acc' where "acc' = w\<^sub>\<pi> l r + missed_\<epsilon> l"
+  obtain l' where l'_def: "buddy r = Some l'"
+   using queue_heap_min_def assms(1)
+   by(auto elim: search_path_cont_condE simp add: r_def)
+define missed' where "missed' = missed_upd (
+                                    missed_upd (missed state) r acc') 
+                                                l' acc'"
+  obtain ben' queue' where ben'_queue'_def:
+   "(ben', queue') = update_best_even_neighbour 
+                                           (abstract_real_map (missed_lookup missed'))
+                                           ben queue l'"
+    using prod.collapse by blast
+  define F' where "F'= extend_forest_even_unclassified F l r l'"
+    define state' where "state' = state \<lparr> forest:= F', 
+                            best_even_neighbour:=ben',
+                            heap:=queue',
+                            missed:=missed',
+                            acc:= acc' \<rparr>"
+    have upd_state_is_state':"search_path_cont_upd state =  state'"
+      using ben'_queue'_def r_def l'_def queue_heap_min_def
+     by(auto simp add: search_path_cont_upd_def state'_def Let_def
+                       F'_def  missed'_def acc'_def l_def ben_def missed_\<epsilon>_def F_def
+                split: option.split prod.split)
+   obtain k where k: "(r, k) \<in> heap_abstract (heap state)"
+        "\<And> x' k'. (x', k') \<in> heap_abstract (heap state) \<Longrightarrow> k \<le> k'"
+     using r_def  pair_eq_fst_snd_eq[OF queue_heap_min_def]
+           heap(5)[of "heap state" r] assms(2)
+     by(auto elim!: invar_basicE)
+   have r_unclassified: "r \<in> Vs G - aevens state - aodds state"
+     using assms(6) k
+     by (auto elim: invar_best_even_neighbour_heapE)
+   have r_l_props: "{r, l} \<in> G" "l \<in> aevens state"
+        "w\<^sub>\<pi> l r + missed_at state l =
+         Min {w\<^sub>\<pi> l r + missed_at state l| l. l \<in> aevens state \<and> {l, r} \<in> G}"
+     using assms(6,7) r_unclassified r_def  k(1) 
+     by(fastforce elim!: invar_best_even_neighbour_mapE 
+                    dest: invar_best_even_neighbour_heapD 
+                simp add: l_def ben_def)+
+   have k_is: "k = w\<^sub>\<pi> l r + missed_at state l"
+     using assms(6) ben_def k(1) l_def
+     by(fastforce dest: invar_best_even_neighbour_heapD)
+   have r_l'_in_M:"{r, l'} \<in> \<M>"
+     using \<M>_def l'_def by fastforce
+   have l'_not_even:"l' \<in> vset_to_set (evens F) \<Longrightarrow> False"
+   proof(goal_cases)
+     case 1
+     hence "{r, l'} \<in> abstract_forest F"
+       using assms(2) evens_and_odds(3)[of \<M> F]  roots(2)[of \<M> F] higher_forest_properties(2)[OF  _ r_l'_in_M, of F] 
+       by(auto elim!: invar_basicE dest!: 
+            simp add: F_def)
+     hence "r \<in> aevens state \<union> aodds state"
+       using  assms(2) 1
+       by(auto elim!: invar_basicE 
+            simp add: F_def higher_forest_properties(3)  insert_commute)
+     thus False
+       using r_unclassified by blast
+   qed
+   have l'_not_even_or_odd:
+      "l' \<in> vset_to_set (evens F) \<union>  vset_to_set (odds F) \<Longrightarrow> False"
+   proof(goal_cases)
+     case 1
+     hence "{r, l'} \<in> abstract_forest F"
+       using assms(2) evens_and_odds(3)[of \<M> F]  roots(2)[of \<M> F] higher_forest_properties(2)[OF  _ r_l'_in_M, of F] 
+       by(auto elim!: invar_basicE dest!: 
+            simp add: F_def)
+     hence "r \<in> aevens state \<union> aodds state"
+       using  assms(2) 1 higher_forest_properties(3)[of \<M> F]
+       by(force elim!: invar_basicE 
+            simp add: F_def   insert_commute)
+     thus False
+       using r_unclassified by blast
+   qed
+    have r_not_even_or_odd:
+      "r \<in> vset_to_set (evens F) \<union>  vset_to_set (odds F) \<Longrightarrow> False"
+   proof(goal_cases)
+     case 1
+     hence "{r, l'} \<in> abstract_forest F"
+       using assms(2) evens_and_odds(3)[of \<M> F]  roots(2)[of \<M> F] higher_forest_properties(2)[OF  _ r_l'_in_M, of F] 
+       by(auto elim!: invar_basicE dest!: 
+            simp add: F_def)
+     hence "r \<in> aevens state \<union> aodds state"
+       using  assms(2) 1 higher_forest_properties(3)[of \<M> F]
+       by(force elim!: invar_basicE 
+            simp add: F_def   insert_commute)
+     thus False
+       using r_unclassified by blast
+   qed
+   have l_r_not_in_M:"{l, r} \<in> \<M> \<Longrightarrow> False" 
+     using r_l_props(2) assms(2) higher_forest_properties(2,3)[of \<M> F l r] 
+           r_not_even_or_odd evens_and_odds(3)[of \<M> F]
+     by(auto elim!: invar_basicE simp add: F_def)
+   have l_in_L:"l \<in> L"
+     using  assms(2) r_l_props(2)
+     by(auto elim!: invar_basicE)
+   hence r_in_R: "r \<in> R"
+     using G(1) bipartite_edgeD(3) l_in_L r_l_props(1) by fastforce
+   moreover have r_l'_in_G:"{r, l'} \<in> G"
+     using l'_def matching(2) by blast
+   ultimately have l'_in_L: "l' \<in> L" 
+     using   bipartite_edgeD(2)[OF _ G(1)]
+     by(auto simp add: insert_commute)
+   have queue'_is: "heap_abstract (fst (heap_extract_min (heap state))) =
+         heap_abstract (heap state) - {(r, w\<^sub>\<pi> l r + missed_at state l)}"
+     using assms(2) k(1) k_is
+     by(intro heap(8))
+       (auto elim!: invar_basicE 
+          simp add: r_def[symmetric] pair_eq_fst_snd_eq[OF queue_heap_min_def])
+   have forest_extension_precond: "forest_extension_precond F \<M> l r l'"
+     using l'_not_even_or_odd r_not_even_or_odd l_r_not_in_M
+     by(auto intro: forest_extension_precondI  
+          simp add: F_def assms(2) invar_basicD(1) r_l_props(2)  r_l'_in_M)
+   have update_best_even_neighbour_conditions:
+        "ben_invar ben" "heap_invar queue" "l' \<in> L"
+        "\<And>r k. (r, k) \<in> heap_abstract queue \<longrightarrow> ben_lookup ben r \<noteq> None"
+        "\<And>r l. ben_lookup ben r = Some l \<longrightarrow>
+          (r, w\<^sub>\<pi> l r + abstract_real_map (missed_lookup missed') l)
+          \<in> heap_abstract queue"
+   proof(goal_cases)
+     case 1
+     then show ?case 
+      using assms(2) ben_def invar_basicD(2) by blast
+   next
+     case 2
+     then show ?case 
+       using heap(2)[OF invar_basicD(3)[OF  assms(2)]] queue_heap_min_def[symmetric] 
+       by simp
+   next
+     case 3
+     then show ?case 
+       using l'_in_L by simp
+   next
+     case (4 rr k)
+     then show ?case 
+     using assms(2,6,7) 
+     by(auto elim!: invar_best_even_neighbour_heapE
+                    invar_best_even_neighbour_mapE invar_basicE
+          simp add: ben_def pair_eq_fst_snd_eq[OF queue_heap_min_def] queue'_is)
+     case (5 rr ll)
+     show ?case 
+     proof(rule, goal_cases)
+       case 1
+       hence "(rr, w\<^sub>\<pi> ll rr + abstract_real_map 
+         (missed_lookup (missed state)) ll) \<in> heap_abstract queue"
+     using assms(2,6,7) 
+     apply(auto elim!: invar_best_even_neighbour_heapE
+                    invar_best_even_neighbour_mapE invar_basicE
+          simp add: ben_def pair_eq_fst_snd_eq[OF queue_heap_min_def] queue'_is missed'_def)
+        apply blast
+     
+     
+   qed
+     using assms(2) ben_def invar_basicD(2) apply bla st
+        apply (met is assms(2) fst_eqD heap(2) invar_basicD(3) queue_heap_min_def)
+     using l'_in_L apply simp
+     using assms(6,7)
+     apply(au to elim!: invar_best_even_neighbour_heapE
+invar_best_even_neighbour_mapE invar_basicE)
+     sledgehammer
+     by simp
+   show "invar_basic (search_path_cont_upd state)"
+     unfolding upd_state_is_state'
+   proof(rule invar_basicI, goal_cases )
+     case 1
+     then show ?case 
+       by(auto intro!: forest_extend(1) 
+            simp add: state'_def F'_def forest_extension_precond)
+   next
+     case 2
+
+     then show ?case
+       using ben'_queue'_def
+       apply(auto simp add: state'_def)
+       using update_best_even_neighbour_correct(1)[OF _ _ _ _ _ ben'_queue'_def]
+       find_theorems update_best_even_neighbour ben_invar
+   next
+     case 3
+     then show ?case sorry
+   next
+     case 4
+     then show ?case sorry
+   next
+     case 5
+     then show ?case sorry
+   next
+     case 6
+     then show ?case sorry
+   next
+     case 7
+     then show ?case sorry
+   next
+     case 8
+     then show ?case sorry
+   qed
+
+
+
+lemma add_to_pot_correct:
+  assumes "potential_invar pot"
+  shows   "potential_invar (add_to_pot pot x val)"
+          "abstract_real_map (potential_lookup (add_to_pot pot x val)) =
+          (\<lambda> y. abstract_real_map (potential_lookup pot) y + (if x = y then val else 0))"
+           "abstract_real_map (potential_lookup (add_to_pot pot x val)) =
+          (\<lambda> y. (if x = y then abstract_real_map (potential_lookup pot) y + val 
+                          else abstract_real_map (potential_lookup pot) y))"
+  using assms
+  by(auto simp add: add_to_pot_def abstract_real_map_def potential(3) 
+          split: option.split
+          intro!: ext 
+           intro: potential(2))
+
+lemma update_best_even_neighbour_correct:
+  assumes "ben_invar ben"
+  shows   "ben_invar (update_best_even_neighbour pot ben l)" (is ?thesis1)
+          "ben_lookup  (update_best_even_neighbour pot ben l) x = None \<Longrightarrow>
+           ben_lookup ben x = None \<and> 
+           \<not> (x \<in> vset_to_set right \<and> {l, x} \<in> G \<and> 
+                  edge_slack pot l x \<le> best_even_neighbour_costs ben x)"
+           (is "?asm2 \<Longrightarrow> ?thesis2")
+          "ben_lookup  (update_best_even_neighbour pot ben l) x = Some (y, sl) \<Longrightarrow>
+           {x, y} \<in> G \<and> slack pot x y = sl \<and> 
+           (\<forall> y' sl'. (({x, y'} \<in> G \<and> sl' = slack pot x y') \<or>
+                        ben_lookup ben x = Some (y', sl')) \<longrightarrow> sl \<le> sl')"
+           (is "?asm3 \<Longrightarrow> ?thesis3")
+proof-
+  define f where "f =  (\<lambda> r ben. if in_G l r
+                 then (if ereal (edge_slack pot l r)
+                            < best_even_neighbour_ereal_costs ben r
+                       then ben_upd ben r (l, edge_slack pot l r)
+                       else ben)
+                 else ben)"
+  define rs where "rs = rev (to_list right)"
+  have to_list_right: "rev (to_list right) = rs" "distinct rs" "vset_to_set right = set rs"
+    using vset(6)[of right] by(auto simp add: rs_def G(4) intro!:vset(5))
+  have invar_one_step: "ben_invar ben \<Longrightarrow> ben_invar (f r ben)" for r ben
+      apply(subst f_def)
+      by(auto intro: best_even_neighbour(2))
+  have invar_iterated: "ben_invar ben \<Longrightarrow> ben_invar (foldr f rs ben)" for rs ben
+  proof(induction rs arbitrary: ben)
+    case (Cons a rs)
+    show ?case 
+      apply(subst foldr_Cons)
+      apply(subst o_apply)
+      by(auto simp add: Cons(2) intro!: Cons(1) invar_one_step best_even_neighbour(2))
+  qed simp
+  show ?thesis1
+    unfolding update_best_even_neighbour_def foldl_conv_foldr
+       f_def[symmetric] 
+    by(auto intro: invar_iterated assms)
+  have non_none_stays_non_none:
+     "\<lbrakk>ben_invar ben; ben_lookup ben x \<noteq> None\<rbrakk> \<Longrightarrow> ben_lookup (f rs ben) x \<noteq> None" for rs ben x
+      apply(subst  f_def)
+      by(auto split: if_split 
+           simp add:  best_even_neighbour(3)
+             intro!: best_even_neighbour(2))
+  have non_none_stays_non_none_list:
+     "\<lbrakk>ben_invar ben; ben_lookup ben x \<noteq> None\<rbrakk> \<Longrightarrow> ben_lookup (foldr f rs ben) x \<noteq> None" for rs ben x
+  proof(induction rs arbitrary: ben)
+    case (Cons a rs)
+    show ?case
+      apply(subst foldr_Cons)
+      apply(subst o_apply)
+      apply(rule non_none_stays_non_none)
+       apply (simp add: Cons.prems(1) invar_iterated)
+      by (simp add: Cons.IH Cons.prems(1,2))
+  qed simp
+
+  have None_one_step: 
+    " ben_lookup ben x = None"
+       "x = a \<Longrightarrow> \<not> ({l, x} \<in> G \<and> edge_slack pot l x \<le> best_even_neighbour_costs ben x)" if 
+    "ben_invar ben""ben_lookup (f a ben) x = None"for ben a x
+    using that
+    apply(all \<open>cases "in_G l a"\<close>)
+    apply(all \<open>cases "ereal (edge_slack pot l a) < best_even_neighbour_ereal_costs ben a"\<close>)
+    apply(all \<open>cases "x = a"\<close>)
+    by(auto simp add: f_def best_even_neighbour(3) G(2) best_even_neighbour_ereal_costs_def)
+  have same_costs_not_in: "\<lbrakk> ben_invar ben; a \<notin> set rs; distinct rs\<rbrakk> 
+ \<Longrightarrow> best_even_neighbour_costs (foldr f rs ben) a = 
+     best_even_neighbour_costs ben a" for a ben
+  proof(induction rs)
+    case (Cons r rs)
+    hence "best_even_neighbour_costs (ben_upd (foldr f rs ben) r (l, edge_slack pot l r)) a
+           = best_even_neighbour_costs  (foldr f rs ben) a"
+      by(auto simp add: best_even_neighbour_costs_def best_even_neighbour(3)  invar_iterated[OF Cons(2), of rs])
+
+    show ?case 
+    apply(subst foldr_Cons, subst o_apply)
+      apply(subst f_def)
+      apply(cases "a = r")
+      using Cons(3)
+       apply(auto split: if_split option.split)
+
+
+
+    find_theorems ben_upd ben_lookup
+
+  show  "?asm2 \<Longrightarrow> ?thesis2"
+ unfolding update_best_even_neighbour_def foldl_conv_foldr
+       f_def[symmetric] to_list_right(1,3)
+  using assms 
+proof(induction rs arbitrary: ben)
+  case (Cons a rs)
+  have ex_unfold:"\<not> (x \<in> set (a # rs) \<and> {l, x} \<in> G \<and>
+        edge_slack pot l x \<le> best_even_neighbour_costs ben x) \<longleftrightarrow>
+       (\<not> (x \<in> set rs \<and> {l, x} \<in> G \<and>
+        edge_slack pot l x \<le> best_even_neighbour_costs ben x) \<and>
+          (x = a \<longrightarrow> \<not> ({l, x} \<in> G \<and> 
+              edge_slack pot l x \<le> best_even_neighbour_costs ben x)))"
+    by auto
+  have ben_invar_later: "ben_invar ((foldr f rs ben) )"
+    by (simp add: assms invar_iterated Cons(3))
+ (* have lookup_after_f_None: "ben_lookup (f a ben) x = None"
+    unfolding f_def
+    apply(auto simp add: best_even_neighbour(3) Cons(3) best_even_neighbour_ereal_costs_def 
+split: if_split option.split)
+
+
+
+
+
+    using non_none_stays_non_none_list[of ben x "a#rs"]
+    using Cons.prems(1,2) ben_invar_later
+           best_even_neighbour(3)
+        fun_upd_other map_upd_Some_unfold
+None_one_step(1)[of "foldr f rs ben" a x]
+
+   
+    unfolding f_def best_even_neighbour_ereal_costs_def  comp_apply  foldr_Cons 
+ 
+    
+
+
+    by (smt (verit, ccfv_SIG))*)
+  show ?case 
+    unfolding  ex_unfold 
+    unfolding conj_assoc[symmetric]
+    apply rule
+    subgoal
+       unfolding conj_assoc
+      apply(rule Cons(1))
+      using Cons(2)
+      by (auto intro: None_one_step(1) ben_invar_later Cons(3))
+    subgoal
+      unfolding conj_assoc
+      apply rule
+      using None_one_step(2)[of "foldr f rs ben" a x]
+      apply (simp add: Cons.prems(2))
+    
+      apply (smt (verit) Cons.prems(1)
+          \<open>ben_lookup ben x = None \<and> \<not> ((x \<in> set rs \<and> {l, x} \<in> G) \<and> edge_slack pot l x \<le> best_even_neighbour_costs ben x)\<close>
+          ben_invar_later best_even_neighbour(3) comp_apply f_def foldr_Cons fun_upd_def
+          not_Some_eq primal_dual_path_search_spec.best_even_neighbour_ereal_costs_def)
+      by simp
+    done
+qed auto
+
+
+      apply(rule Suc(1))
+      subgoal
+        using Suc(2)[simplified rs_is(1)]
+        apply(subst (asm) foldl_Cons)
+        apply(subst (asm) (2) f_def)
+        apply(all \<open>cases "in_G a r"\<close>)
+        apply(all \<open>cases "ereal (edge_slack pot a r) < best_even_neighbour_ereal_costs ben r"\<close>)
+           apply auto
+        term fold
+
+    unfolding 
+    using conjunct1[OF Suc(1), of ben]
+    unfolding foldl_Cons
+    using non_none_stays_non_none
+    using conjunct1[OF Suc(1), of ben]
+
+    using non_none_stays_non_none[of]
+       apply(au to simp add: f_def)
+    using non_none_stays_non_none
+    
+   
+qed auto
+
+    find_theorems to_list
+
+
+
+
+
+
+
+
+
+
+
+
+
+
+
+
+
+  oops
+
+    and best_even_neighb_empty::"'ben"
+    and best_even_neighb_upd::"'ben \<Rightarrow> 'v \<Rightarrow> ('v \<times> real) \<Rightarrow> 'ben"
+    and best_even_neighb_lookup::"'ben \<Rightarrow> 'v \<Rightarrow> ('v \<times> real)"
+
    and vset_empty::'vset
    and vset_insert::"'v \<Rightarrow> 'vset \<Rightarrow>'vset"
    and vset_invar::"'vset \<Rightarrow> bool"
